CoqOfRust/move_sui/simulations/move_bytecode_verifier/type_safety_tests/mod.v
@@ -2330,3 +2330,5065 @@ Goal
   exists (Error : Set) (error : Error),
   test_unpack_no_arg = panic! error.
 Proof. repeat eexists. Qed.
+
+(*
+#[test]
+fn test_unpack_generic_correct_types() {
+    let code = vec![
+        Bytecode::LdU32(42),
+        Bytecode::PackGeneric(StructDefInstantiationIndex(0)),
+        Bytecode::UnpackGeneric(StructDefInstantiationIndex(0)),
+    ];
+    let mut module: CompiledModule = make_module(code);
+    add_simple_struct_generic_with_abilities(
+        &mut module,
+        AbilitySet::PRIMITIVES,
+        SignatureToken::U32,
+    );
+    let fun_context = get_fun_context(&module);
+    let result = type_safety::verify(&module, &fun_context, &mut DummyMeter);
+    assert!(result.is_ok());
+}
+*)
+Definition test_unpack_generic_correct_types : M!? PartialVMError.t unit :=
+  let code := [
+    Bytecode.LdU32 42;
+    Bytecode.PackGeneric (StructDefInstantiationIndex.Build_t 0);
+    Bytecode.UnpackGeneric (StructDefInstantiationIndex.Build_t 0)
+  ] in
+  let module := make_module code in
+  let module := add_simple_struct_generic_with_abilities
+    module AbilitySet.PRIMITIVES SignatureToken.U32 in
+  let! fun_context := get_fun_context module in
+  verify module fun_context.
+
+Goal test_unpack_generic_correct_types = return!? tt.
+Proof. reflexivity. Qed.
+
+(*
+#[test]
+fn test_unpack_generic_wrong_type() {
+    let code = vec![
+        Bytecode::LdU32(42),
+        Bytecode::UnpackGeneric(StructDefInstantiationIndex(0)),
+    ];
+    let mut module: CompiledModule = make_module(code);
+    add_simple_struct_generic_with_abilities(
+        &mut module,
+        AbilitySet::PRIMITIVES,
+        SignatureToken::U32,
+    );
+    let fun_context = get_fun_context(&module);
+    let result = type_safety::verify(&module, &fun_context, &mut DummyMeter);
+    assert_eq!(
+        result.unwrap_err().major_status(),
+        StatusCode::UNPACK_TYPE_MISMATCH_ERROR
+    );
+}
+*)
+Definition test_unpack_generic_wrong_type : M! unit :=
+  let code := [
+    Bytecode.LdU32 42;
+    Bytecode.UnpackGeneric (StructDefInstantiationIndex.Build_t 0)
+  ] in
+  let module := make_module code in
+  let module := add_simple_struct_generic_with_abilities
+    module AbilitySet.PRIMITIVES SignatureToken.U32 in
+  let! fun_context := get_fun_context module in
+  assert_major_status
+    (verify module fun_context)
+    (fun status =>
+      match status with
+      | StatusCode.UNPACK_TYPE_MISMATCH_ERROR => true
+      | _ => false
+      end
+    ).
+
+Goal test_unpack_generic_wrong_type = return! tt.
+Proof. reflexivity. Qed.
+
+(*
+#[test]
+#[should_panic]
+fn test_unpack_generic_no_arg() {
+    let code = vec![Bytecode::UnpackGeneric(StructDefInstantiationIndex(0))];
+    let mut module: CompiledModule = make_module(code);
+    add_simple_struct_generic_with_abilities(
+        &mut module,
+        AbilitySet::PRIMITIVES,
+        SignatureToken::U32,
+    );
+    let fun_context = get_fun_context(&module);
+    let _result = type_safety::verify(&module, &fun_context, &mut DummyMeter);
+}
+*)
+Definition test_unpack_generic_no_arg : M!? _ unit :=
+  let code := [Bytecode.UnpackGeneric (StructDefInstantiationIndex.Build_t 0)] in
+  let module := make_module code in
+  let module := add_simple_struct_generic_with_abilities
+    module AbilitySet.PRIMITIVES SignatureToken.U32 in
+  let! fun_context := get_fun_context module in
+  verify module fun_context.
+
+Goal
+  exists (Error : Set) (error : Error),
+  test_unpack_generic_no_arg = panic! error.
+Proof. repeat eexists. Qed.
+
+(*
+#[test]
+fn test_eq_neq_correct_types() {
+    for instr in vec![Bytecode::Eq, Bytecode::Neq] {
+        let code = vec![Bytecode::LdU32(42), Bytecode::LdU32(42), instr.clone()];
+        let module = make_module(code);
+        let fun_context = get_fun_context(&module);
+        let result = type_safety::verify(&module, &fun_context, &mut DummyMeter);
+        assert!(result.is_ok());
+
+        let code = vec![
+            Bytecode::LdU32(42),
+            Bytecode::Pack(StructDefinitionIndex(0)),
+            Bytecode::LdU32(51),
+            Bytecode::Pack(StructDefinitionIndex(0)),
+            instr.clone(),
+        ];
+        let mut module = make_module(code);
+        add_simple_struct_with_abilities(&mut module, AbilitySet::PRIMITIVES);
+        let fun_context = get_fun_context(&module);
+        let result = type_safety::verify(&module, &fun_context, &mut DummyMeter);
+        assert!(result.is_ok());
+    }
+}
+*)
+Definition test_eq_neq_correct_types
+    (instr : Bytecode.t) :
+    M!? PartialVMError.t unit :=
+  let code := [Bytecode.LdU32 42; Bytecode.LdU32 42; instr] in
+  let module := make_module code in
+  let! fun_context := get_fun_context module in
+  let! result := verify module fun_context in
+  let code := [
+    Bytecode.LdU32 42;
+    Bytecode.Pack (StructDefinitionIndex.Build_t 0);
+    Bytecode.LdU32 51;
+    Bytecode.Pack (StructDefinitionIndex.Build_t 0);
+    instr
+  ] in
+  let module := make_module code in
+  let module := add_simple_struct_with_abilities module AbilitySet.PRIMITIVES in
+  let! fun_context := get_fun_context module in
+  verify module fun_context.
+
+Goal List.Forall
+  (fun instr => test_eq_neq_correct_types instr = return!? tt)
+  [
+    Bytecode.Eq;
+    Bytecode.Neq
+  ].
+Proof. repeat constructor. Qed.
+
+(*
+#[test]
+fn test_eq_neq_mismatched_types() {
+    for instr in vec![Bytecode::Eq, Bytecode::Neq] {
+        let code = vec![Bytecode::LdU32(42), Bytecode::LdU64(42), instr.clone()];
+        let module = make_module(code);
+        let fun_context = get_fun_context(&module);
+        let result = type_safety::verify(&module, &fun_context, &mut DummyMeter);
+        assert_eq!(
+            result.unwrap_err().major_status(),
+            StatusCode::EQUALITY_OP_TYPE_MISMATCH_ERROR
+        );
+    }
+}
+*)
+Definition test_eq_neq_mismatched_types
+    (instr : Bytecode.t) :
+    M! unit :=
+  let code := [Bytecode.LdU32 42; Bytecode.LdU64 42; instr] in
+  let module := make_module code in
+  let! fun_context := get_fun_context module in
+  assert_major_status
+    (verify module fun_context)
+    (fun status =>
+      match status with
+      | StatusCode.EQUALITY_OP_TYPE_MISMATCH_ERROR => true
+      | _ => false
+      end
+    ).
+
+Goal List.Forall
+  (fun instr => test_eq_neq_mismatched_types instr = return! tt)
+  [
+    Bytecode.Eq;
+    Bytecode.Neq
+  ].
+Proof. repeat constructor. Qed.
+
+(*
+#[test]
+fn test_eq_neq_no_drop() {
+    for instr in vec![Bytecode::Eq, Bytecode::Neq] {
+        let code = vec![
+            Bytecode::LdU32(42),
+            Bytecode::Pack(StructDefinitionIndex(0)),
+            Bytecode::LdU32(51),
+            Bytecode::Pack(StructDefinitionIndex(0)),
+            instr.clone(),
+        ];
+
+        let mut module = make_module(code);
+        add_simple_struct_with_abilities(&mut module, AbilitySet::EMPTY);
+        let fun_context = get_fun_context(&module);
+        let result = type_safety::verify(&module, &fun_context, &mut DummyMeter);
+        assert_eq!(
+            result.unwrap_err().major_status(),
+            StatusCode::EQUALITY_OP_TYPE_MISMATCH_ERROR
+        );
+    }
+}
+*)
+Definition test_eq_neq_no_drop
+    (instr : Bytecode.t) :
+    M! unit :=
+  let code := [
+    Bytecode.LdU32 42;
+    Bytecode.Pack (StructDefinitionIndex.Build_t 0);
+    Bytecode.LdU32 51;
+    Bytecode.Pack (StructDefinitionIndex.Build_t 0);
+    instr
+  ] in
+  let module := make_module code in
+  let module := add_simple_struct_with_abilities module AbilitySet.EMPTY in
+  let! fun_context := get_fun_context module in
+  assert_major_status
+    (verify module fun_context)
+    (fun status =>
+      match status with
+      | StatusCode.EQUALITY_OP_TYPE_MISMATCH_ERROR => true
+      | _ => false
+      end
+    ).
+
+Goal List.Forall
+  (fun instr => test_eq_neq_no_drop instr = return! tt)
+  [
+    Bytecode.Eq;
+    Bytecode.Neq
+  ].
+Proof. repeat constructor. Qed.
+
+(*
+#[test]
+#[should_panic]
+fn test_eq_neq_too_few_args() {
+    for instr in vec![Bytecode::Eq, Bytecode::Neq] {
+        let code = vec![Bytecode::LdU32(42), instr.clone()];
+        let module = make_module(code);
+        let fun_context = get_fun_context(&module);
+        let _result = type_safety::verify(&module, &fun_context, &mut DummyMeter);
+    }
+}
+*)
+Definition test_eq_neq_too_few_args
+    (instr : Bytecode.t) :
+    M!? _ unit :=
+  let code := [Bytecode.LdU32 42; instr] in
+  let module := make_module code in
+  let! fun_context := get_fun_context module in
+  verify module fun_context.
+
+Goal List.Forall
+  (fun instr =>
+    exists (Error : Set) (error : Error),
+    test_eq_neq_too_few_args instr = panic! error
+  )
+  [
+    Bytecode.Eq;
+    Bytecode.Neq
+  ].
+Proof. repeat constructor; repeat eexists. Qed.
+
+(*
+#[test]
+#[should_panic]
+fn test_eq_neq_no_args() {
+    for instr in vec![Bytecode::Eq, Bytecode::Neq] {
+        let code = vec![instr.clone()];
+        let module = make_module(code);
+        let fun_context = get_fun_context(&module);
+        let _result = type_safety::verify(&module, &fun_context, &mut DummyMeter);
+    }
+}
+*)
+Definition test_eq_neq_no_args
+    (instr : Bytecode.t) :
+    M!? _ unit :=
+  let code := [instr] in
+  let module := make_module code in
+  let! fun_context := get_fun_context module in
+  verify module fun_context.
+
+Goal List.Forall
+  (fun instr =>
+    exists (Error : Set) (error : Error),
+    test_eq_neq_no_args instr = panic! error
+  )
+  [
+    Bytecode.Eq;
+    Bytecode.Neq
+  ].
+Proof. repeat constructor; repeat eexists. Qed.
+
+(*
+#[test]
+fn test_pop_ok() {
+    let code = vec![Bytecode::LdU32(42), Bytecode::Pop];
+    let module = make_module(code);
+    let fun_context = get_fun_context(&module);
+    let result = type_safety::verify(&module, &fun_context, &mut DummyMeter);
+    assert!(result.is_ok());
+}
+*)
+Definition test_pop_ok : M!? PartialVMError.t unit :=
+  let code := [Bytecode.LdU32 42; Bytecode.Pop] in
+  let module := make_module code in
+  let! fun_context := get_fun_context module in
+  verify module fun_context.
+
+Goal test_pop_ok = return!? tt.
+Proof. reflexivity. Qed.
+
+(*
+#[test]
+fn test_pop_no_drop() {
+    let code = vec![
+        Bytecode::LdU32(42),
+        Bytecode::Pack(StructDefinitionIndex(0)),
+        Bytecode::Pop,
+    ];
+    let mut module = make_module(code);
+    add_simple_struct_with_abilities(&mut module, AbilitySet::EMPTY);
+    let fun_context = get_fun_context(&module);
+    let result = type_safety::verify(&module, &fun_context, &mut DummyMeter);
+    assert_eq!(
+        result.unwrap_err().major_status(),
+        StatusCode::POP_WITHOUT_DROP_ABILITY
+    );
+}
+*)
+Definition test_pop_no_drop : M! unit :=
+  let code := [
+    Bytecode.LdU32 42;
+    Bytecode.Pack (StructDefinitionIndex.Build_t 0);
+    Bytecode.Pop
+  ] in
+  let module := make_module code in
+  let module := add_simple_struct_with_abilities module AbilitySet.EMPTY in
+  let! fun_context := get_fun_context module in
+  assert_major_status
+    (verify module fun_context)
+    (fun status =>
+      match status with
+      | StatusCode.POP_WITHOUT_DROP_ABILITY => true
+      | _ => false
+      end
+    ).
+
+Goal test_pop_no_drop = return! tt.
+Proof. reflexivity. Qed.
+
+(*
+#[test]
+#[should_panic]
+fn test_pop_no_arg() {
+    let code = vec![Bytecode::Pop];
+    let module = make_module(code);
+    let fun_context = get_fun_context(&module);
+    let _result = type_safety::verify(&module, &fun_context, &mut DummyMeter);
+}
+*)
+Definition test_pop_no_arg : M!? _ unit :=
+  let code := [Bytecode.Pop] in
+  let module := make_module code in
+  let! fun_context := get_fun_context module in
+  verify module fun_context.
+
+Goal
+  exists (Error : Set) (error : Error),
+  test_pop_no_arg = panic! error.
+Proof. repeat eexists. Qed.
+
+(*
+#[test]
+fn test_borrow_loc_ok() {
+    for instr in vec![Bytecode::ImmBorrowLoc(1), Bytecode::MutBorrowLoc(0)] {
+        let code = vec![instr];
+        let module = make_module_with_local(code, SignatureToken::U64);
+        let fun_context = get_fun_context(&module);
+        let result = type_safety::verify(&module, &fun_context, &mut DummyMeter);
+        assert!(result.is_ok());
+    }
+}
+*)
+Definition test_borrow_loc_ok
+    (instr : Bytecode.t) :
+    M!? PartialVMError.t unit :=
+  let code := [instr] in
+  let module := make_module_with_local code SignatureToken.U64 in
+  let! fun_context := get_fun_context module in
+  verify module fun_context.
+
+Goal List.Forall
+  (fun instr => test_borrow_loc_ok instr = return!? tt)
+  [
+    Bytecode.ImmBorrowLoc 1;
+    Bytecode.MutBorrowLoc 0
+  ].
+Proof. repeat constructor. Qed.
+
+(*
+#[test]
+fn test_borrow_loc_reference() {
+    for instr in vec![Bytecode::ImmBorrowLoc(1), Bytecode::MutBorrowLoc(0)] {
+        for reference in vec![
+            SignatureToken::Reference(Box::new(SignatureToken::U64)),
+            SignatureToken::MutableReference(Box::new(SignatureToken::U32)),
+        ] {
+            let code = vec![instr.clone()];
+            let module = make_module_with_local(code, reference.clone());
+            let fun_context = get_fun_context(&module);
+            let result = type_safety::verify(&module, &fun_context, &mut DummyMeter);
+            assert_eq!(
+                result.unwrap_err().major_status(),
+                StatusCode::BORROWLOC_REFERENCE_ERROR
+            );
+        }
+    }
+}
+*)
+Definition test_borrow_loc_reference
+    (instr : Bytecode.t)
+    (reference : SignatureToken.t) :
+    M! unit :=
+  let code := [instr] in
+  let module := make_module_with_local code reference in
+  let! fun_context := get_fun_context module in
+  assert_major_status
+    (verify module fun_context)
+    (fun status =>
+      match status with
+      | StatusCode.BORROWLOC_REFERENCE_ERROR => true
+      | _ => false
+      end
+    ).
+
+Goal List.Forall
+  (fun instr =>
+    List.Forall
+      (fun reference =>
+        test_borrow_loc_reference instr reference = return! tt
+      )
+      [
+        SignatureToken.Reference (SignatureToken.U64);
+        SignatureToken.MutableReference (SignatureToken.U32)
+      ]
+  )
+  [
+    Bytecode.ImmBorrowLoc 1;
+    Bytecode.MutBorrowLoc 0
+  ].
+Proof.
+  repeat constructor.
+Qed.
+
+(*
+#[test]
+fn test_st_lock_correct_type() {
+    let code = vec![Bytecode::LdU32(51), Bytecode::StLoc(0)];
+    let module = make_module_with_local(code, SignatureToken::U32);
+    let fun_context = get_fun_context(&module);
+    let result = type_safety::verify(&module, &fun_context, &mut DummyMeter);
+    assert!(result.is_ok());
+}
+*)
+Definition test_st_lock_correct_type : M!? PartialVMError.t unit :=
+  let code := [Bytecode.LdU32 51; Bytecode.StLoc 0] in
+  let module := make_module_with_local code SignatureToken.U32 in
+  let! fun_context := get_fun_context module in
+  verify module fun_context.
+
+Goal test_st_lock_correct_type = return!? tt.
+Proof. reflexivity. Qed.
+
+(*
+#[test]
+fn test_st_lock_mismatched_types() {
+    let code = vec![Bytecode::LdU64(51), Bytecode::StLoc(0)];
+    let module = make_module_with_local(code, SignatureToken::U32);
+    let fun_context = get_fun_context(&module);
+    let result = type_safety::verify(&module, &fun_context, &mut DummyMeter);
+    assert_eq!(
+        result.unwrap_err().major_status(),
+        StatusCode::STLOC_TYPE_MISMATCH_ERROR
+    );
+}
+*)
+Definition test_st_lock_mismatched_types : M! unit :=
+  let code := [Bytecode.LdU64 51; Bytecode.StLoc 0] in
+  let module := make_module_with_local code SignatureToken.U32 in
+  let! fun_context := get_fun_context module in
+  assert_major_status
+    (verify module fun_context)
+    (fun status =>
+      match status with
+      | StatusCode.STLOC_TYPE_MISMATCH_ERROR => true
+      | _ => false
+      end
+    ).
+
+Goal test_st_lock_mismatched_types = return! tt.
+Proof.
+  reflexivity.
+Qed.
+
+(*
+#[test]
+#[should_panic]
+fn test_st_lock_no_arg() {
+    let code = vec![Bytecode::StLoc(0)];
+    let module = make_module_with_local(code, SignatureToken::U32);
+    let fun_context = get_fun_context(&module);
+    let _result = type_safety::verify(&module, &fun_context, &mut DummyMeter);
+}
+*)
+Definition test_st_lock_no_arg : M!? _ unit :=
+  let code := [Bytecode.StLoc 0] in
+  let module := make_module_with_local code SignatureToken.U32 in
+  let! fun_context := get_fun_context module in
+  verify module fun_context.
+
+Goal
+  exists (Error : Set) (error : Error),
+  test_st_lock_no_arg = panic! error.
+Proof. repeat eexists. Qed.
+
+(*
+#[test]
+fn test_copy_loc_ok() {
+    let code = vec![Bytecode::CopyLoc(0)];
+    let module = make_module_with_local(code, SignatureToken::U64);
+    let fun_context = get_fun_context(&module);
+    let result = type_safety::verify(&module, &fun_context, &mut DummyMeter);
+    assert!(result.is_ok());
+}
+*)
+Definition test_copy_loc_ok : M!? PartialVMError.t unit :=
+  let code := [Bytecode.CopyLoc 0] in
+  let module := make_module_with_local code SignatureToken.U64 in
+  let! fun_context := get_fun_context module in
+  verify module fun_context.
+
+Goal test_copy_loc_ok = return!? tt.
+Proof. reflexivity. Qed.
+
+(*
+#[test]
+fn test_copy_loc_no_copy() {
+    let code = vec![Bytecode::CopyLoc(0)];
+    let mut module = make_module_with_local(code, SignatureToken::Struct(StructHandleIndex(0)));
+    add_simple_struct_with_abilities(&mut module, AbilitySet::EMPTY);
+    let fun_context = get_fun_context(&module);
+    let result = type_safety::verify(&module, &fun_context, &mut DummyMeter);
+    assert_eq!(
+        result.unwrap_err().major_status(),
+        StatusCode::COPYLOC_WITHOUT_COPY_ABILITY
+    );
+}
+*)
+Definition test_copy_loc_no_copy : M! unit :=
+  let code := [Bytecode.CopyLoc 0] in
+  let module := make_module_with_local code (SignatureToken.Struct (StructHandleIndex.Build_t 0)) in
+  let module := add_simple_struct_with_abilities module AbilitySet.EMPTY in
+  let! fun_context := get_fun_context module in
+  assert_major_status
+    (verify module fun_context)
+    (fun status =>
+      match status with
+      | StatusCode.COPYLOC_WITHOUT_COPY_ABILITY => true
+      | _ => false
+      end
+    ).
+
+Goal test_copy_loc_no_copy = return! tt.
+Proof. reflexivity. Qed.
+
+(*
+#[test]
+fn test_move_loc_ok() {
+    let code = vec![Bytecode::MoveLoc(0)];
+    let module = make_module_with_local(code, SignatureToken::U64);
+    let fun_context = get_fun_context(&module);
+    let result = type_safety::verify(&module, &fun_context, &mut DummyMeter);
+    assert!(result.is_ok());
+}
+*)
+Definition test_move_loc_ok : M!? PartialVMError.t unit :=
+  let code := [Bytecode.MoveLoc 0] in
+  let module := make_module_with_local code SignatureToken.U64 in
+  let! fun_context := get_fun_context module in
+  verify module fun_context.
+
+Goal test_move_loc_ok = return!? tt.
+Proof. reflexivity. Qed.
+
+(*
+#[test]
+fn test_freeze_ref_correct_type() {
+    let code = vec![Bytecode::MutBorrowLoc(0), Bytecode::FreezeRef];
+    let module = make_module_with_local(code, SignatureToken::U64);
+    let fun_context = get_fun_context(&module);
+    let result = type_safety::verify(&module, &fun_context, &mut DummyMeter);
+    assert!(result.is_ok());
+}
+*)
+Definition test_freeze_ref_correct_type : M!? PartialVMError.t unit :=
+  let code := [Bytecode.MutBorrowLoc 0; Bytecode.FreezeRef] in
+  let module := make_module_with_local code SignatureToken.U64 in
+  let! fun_context := get_fun_context module in
+  verify module fun_context.
+
+Goal test_freeze_ref_correct_type = return!? tt.
+Proof. reflexivity. Qed.
+
+(*
+#[test]
+fn test_freeze_ref_wrong_type() {
+    let code = vec![Bytecode::ImmBorrowLoc(0), Bytecode::FreezeRef];
+    let module = make_module_with_local(code, SignatureToken::U64);
+    let fun_context = get_fun_context(&module);
+    let result = type_safety::verify(&module, &fun_context, &mut DummyMeter);
+    assert_eq!(
+        result.unwrap_err().major_status(),
+        StatusCode::FREEZEREF_TYPE_MISMATCH_ERROR
+    );
+
+    let code = vec![Bytecode::LdTrue, Bytecode::FreezeRef];
+    let module = make_module_with_local(code, SignatureToken::U64);
+    let fun_context = get_fun_context(&module);
+    let result = type_safety::verify(&module, &fun_context, &mut DummyMeter);
+    assert_eq!(
+        result.unwrap_err().major_status(),
+        StatusCode::FREEZEREF_TYPE_MISMATCH_ERROR
+    );
+}
+*)
+Definition test_freeze_ref_wrong_type : M! unit :=
+  let code := [Bytecode.ImmBorrowLoc 0; Bytecode.FreezeRef] in
+  let module := make_module_with_local code SignatureToken.U64 in
+  let! fun_context := get_fun_context module in
+  do! assert_major_status
+    (verify module fun_context)
+    (fun status =>
+      match status with
+      | StatusCode.FREEZEREF_TYPE_MISMATCH_ERROR => true
+      | _ => false
+      end
+    ) in
+  let code := [Bytecode.LdTrue; Bytecode.FreezeRef] in
+  let module := make_module_with_local code SignatureToken.U64 in
+  let! fun_context := get_fun_context module in
+  assert_major_status
+    (verify module fun_context)
+    (fun status =>
+      match status with
+      | StatusCode.FREEZEREF_TYPE_MISMATCH_ERROR => true
+      | _ => false
+      end
+    ).
+
+Goal test_freeze_ref_wrong_type = return! tt.
+Proof. reflexivity. Qed.
+
+(*
+#[test]
+#[should_panic]
+fn test_freeze_ref_no_arg() {
+    let code = vec![Bytecode::FreezeRef];
+    let module = make_module_with_local(code, SignatureToken::U64);
+    let fun_context = get_fun_context(&module);
+    let _result = type_safety::verify(&module, &fun_context, &mut DummyMeter);
+}
+*)
+Definition test_freeze_ref_no_arg : M!? _ unit :=
+  let code := [Bytecode.FreezeRef] in
+  let module := make_module_with_local code SignatureToken.U64 in
+  let! fun_context := get_fun_context module in
+  verify module fun_context.
+
+Goal
+  exists (Error : Set) (error : Error),
+  test_freeze_ref_no_arg = panic! error.
+Proof. repeat eexists. Qed.
+
+(*
+#[test]
+fn test_read_ref_correct_type() {
+    for instr in vec![Bytecode::ImmBorrowLoc(0), Bytecode::MutBorrowLoc(0)] {
+        let code = vec![instr, Bytecode::ReadRef];
+        let module = make_module_with_local(code, SignatureToken::U64);
+        let fun_context = get_fun_context(&module);
+        let result = type_safety::verify(&module, &fun_context, &mut DummyMeter);
+        assert!(result.is_ok());
+    }
+}
+*)
+Definition test_read_ref_correct_type
+    (instr : Bytecode.t) :
+    M!? PartialVMError.t unit :=
+  let code := [instr; Bytecode.ReadRef] in
+  let module := make_module_with_local code SignatureToken.U64 in
+  let! fun_context := get_fun_context module in
+  verify module fun_context.
+
+Goal List.Forall
+  (fun instr => test_read_ref_correct_type instr = return!? tt)
+  [
+    Bytecode.ImmBorrowLoc 0;
+    Bytecode.MutBorrowLoc 0
+  ].
+Proof. repeat constructor. Qed.
+
+(*
+#[test]
+fn test_read_ref_wrong_type() {
+    let code = vec![Bytecode::LdU64(42), Bytecode::ReadRef];
+    let module = make_module_with_local(code, SignatureToken::U64);
+    let fun_context = get_fun_context(&module);
+    let result = type_safety::verify(&module, &fun_context, &mut DummyMeter);
+    assert_eq!(
+        result.unwrap_err().major_status(),
+        StatusCode::READREF_TYPE_MISMATCH_ERROR
+    );
+}
+*)
+Definition test_read_ref_wrong_type : M! unit :=
+  let code := [Bytecode.LdU64 42; Bytecode.ReadRef] in
+  let module := make_module_with_local code SignatureToken.U64 in
+  let! fun_context := get_fun_context module in
+  assert_major_status
+    (verify module fun_context)
+    (fun status =>
+      match status with
+      | StatusCode.READREF_TYPE_MISMATCH_ERROR => true
+      | _ => false
+      end
+    ).
+
+Goal test_read_ref_wrong_type = return! tt.
+Proof. reflexivity. Qed.
+
+(*
+#[test]
+fn test_read_ref_no_copy() {
+    for instr in vec![Bytecode::ImmBorrowLoc(0), Bytecode::MutBorrowLoc(0)] {
+        let code = vec![instr, Bytecode::ReadRef];
+        let mut module = make_module_with_local(code, SignatureToken::Struct(StructHandleIndex(0)));
+        add_simple_struct_with_abilities(&mut module, AbilitySet::EMPTY);
+        let fun_context = get_fun_context(&module);
+        let result = type_safety::verify(&module, &fun_context, &mut DummyMeter);
+        assert_eq!(
+            result.unwrap_err().major_status(),
+            StatusCode::READREF_WITHOUT_COPY_ABILITY
+        );
+    }
+}
+*)
+Definition test_read_ref_no_copy (instr : Bytecode.t) : M! unit :=
+  let code := [instr; Bytecode.ReadRef] in
+  let module := make_module_with_local code (SignatureToken.Struct (StructHandleIndex.Build_t 0)) in
+  let module := add_simple_struct_with_abilities module AbilitySet.EMPTY in
+  let! fun_context := get_fun_context module in
+  assert_major_status
+    (verify module fun_context)
+    (fun status =>
+      match status with
+      | StatusCode.READREF_WITHOUT_COPY_ABILITY => true
+      | _ => false
+      end
+    ).
+
+Goal List.Forall
+  (fun instr => test_read_ref_no_copy instr = return! tt)
+  [
+    Bytecode.ImmBorrowLoc 0;
+    Bytecode.MutBorrowLoc 0
+  ].
+Proof. repeat constructor. Qed.
+
+(*
+#[test]
+#[should_panic]
+fn test_read_ref_no_arg() {
+    let code = vec![Bytecode::ReadRef];
+    let module = make_module_with_local(code, SignatureToken::U64);
+    let fun_context = get_fun_context(&module);
+    let _result = type_safety::verify(&module, &fun_context, &mut DummyMeter);
+}
+*)
+Definition test_read_ref_no_arg : M!? _ unit :=
+  let code := [Bytecode.ReadRef] in
+  let module := make_module_with_local code SignatureToken.U64 in
+  let! fun_context := get_fun_context module in
+  verify module fun_context.
+
+Goal
+  exists (Error : Set) (error : Error),
+  test_read_ref_no_arg = panic! error.
+Proof. repeat eexists. Qed.
+
+(*
+#[test]
+fn test_write_ref_correct_type() {
+    let code = vec![
+        Bytecode::LdU64(42),
+        Bytecode::MutBorrowLoc(0),
+        Bytecode::WriteRef,
+    ];
+    let module = make_module_with_local(code, SignatureToken::U64);
+    let fun_context = get_fun_context(&module);
+    let result = type_safety::verify(&module, &fun_context, &mut DummyMeter);
+    assert!(result.is_ok());
+
+    let code = vec![
+        Bytecode::LdU32(42),
+        Bytecode::Pack(StructDefinitionIndex(0)),
+        Bytecode::MutBorrowLoc(0),
+        Bytecode::WriteRef,
+    ];
+    let mut module = make_module_with_local(code, SignatureToken::Struct(StructHandleIndex(0)));
+    add_simple_struct_with_abilities(&mut module, AbilitySet::PRIMITIVES);
+    let fun_context = get_fun_context(&module);
+    let result = type_safety::verify(&module, &fun_context, &mut DummyMeter);
+    assert!(result.is_ok());
+}
+*)
+Definition test_write_ref_correct_type : M! unit :=
+  let code := [
+    Bytecode.LdU64 42;
+    Bytecode.MutBorrowLoc 0;
+    Bytecode.WriteRef
+  ] in
+  let module := make_module_with_local code SignatureToken.U64 in
+  let! fun_context := get_fun_context module in
+  let! result := verify module fun_context in
+  do! assert_is_ok result in
+  let code := [
+    Bytecode.LdU32 42;
+    Bytecode.Pack (StructDefinitionIndex.Build_t 0);
+    Bytecode.MutBorrowLoc 0;
+    Bytecode.WriteRef
+  ] in
+  let module := make_module_with_local code (SignatureToken.Struct (StructHandleIndex.Build_t 0)) in
+  let module := add_simple_struct_with_abilities module AbilitySet.PRIMITIVES in
+  let! fun_context := get_fun_context module in
+  let! result := verify module fun_context in
+  assert_is_ok result.
+
+Goal test_write_ref_correct_type = return! tt.
+Proof.
+  reflexivity.
+Qed.
+
+(*
+#[test]
+fn test_write_ref_wrong_type() {
+    let code = vec![
+        Bytecode::LdU64(42),
+        Bytecode::ImmBorrowLoc(0),
+        Bytecode::WriteRef,
+    ];
+    let module = make_module_with_local(code, SignatureToken::U64);
+    let fun_context = get_fun_context(&module);
+    let result = type_safety::verify(&module, &fun_context, &mut DummyMeter);
+    assert_eq!(
+        result.unwrap_err().major_status(),
+        StatusCode::WRITEREF_NO_MUTABLE_REFERENCE_ERROR
+    );
+}
+*)
+Definition test_write_ref_wrong_type : M! unit :=
+  let code := [
+    Bytecode.LdU64 42;
+    Bytecode.ImmBorrowLoc 0;
+    Bytecode.WriteRef
+  ] in
+  let module := make_module_with_local code SignatureToken.U64 in
+  let! fun_context := get_fun_context module in
+  assert_major_status
+    (verify module fun_context)
+    (fun status =>
+      match status with
+      | StatusCode.WRITEREF_NO_MUTABLE_REFERENCE_ERROR => true
+      | _ => false
+      end
+    ).
+
+Goal test_write_ref_wrong_type = return! tt.
+Proof. reflexivity. Qed.
+
+(*
+#[test]
+fn test_write_ref_mismatched_types() {
+    let code = vec![
+        Bytecode::LdU32(42),
+        Bytecode::MutBorrowLoc(0),
+        Bytecode::WriteRef,
+    ];
+    let module = make_module_with_local(code, SignatureToken::U64);
+    let fun_context = get_fun_context(&module);
+    let result = type_safety::verify(&module, &fun_context, &mut DummyMeter);
+    assert_eq!(
+        result.unwrap_err().major_status(),
+        StatusCode::WRITEREF_TYPE_MISMATCH_ERROR
+    );
+}
+*)
+Definition test_write_ref_mismatched_types : M! unit :=
+  let code := [
+    Bytecode.LdU32 42;
+    Bytecode.MutBorrowLoc 0;
+    Bytecode.WriteRef
+  ] in
+  let module := make_module_with_local code SignatureToken.U64 in
+  let! fun_context := get_fun_context module in
+  assert_major_status
+    (verify module fun_context)
+    (fun status =>
+      match status with
+      | StatusCode.WRITEREF_TYPE_MISMATCH_ERROR => true
+      | _ => false
+      end
+    ).
+
+Goal test_write_ref_mismatched_types = return! tt.
+Proof. reflexivity. Qed.
+
+(*
+#[test]
+fn test_write_ref_no_drop() {
+    let code = vec![
+        Bytecode::LdU32(42),
+        Bytecode::Pack(StructDefinitionIndex(0)),
+        Bytecode::MutBorrowLoc(0),
+        Bytecode::WriteRef,
+    ];
+    let mut module = make_module_with_local(code, SignatureToken::Struct(StructHandleIndex(0)));
+    add_simple_struct_with_abilities(&mut module, AbilitySet::EMPTY);
+    let fun_context = get_fun_context(&module);
+    let result = type_safety::verify(&module, &fun_context, &mut DummyMeter);
+    assert_eq!(
+        result.unwrap_err().major_status(),
+        StatusCode::WRITEREF_WITHOUT_DROP_ABILITY
+    );
+}
+*)
+Definition test_write_ref_no_drop : M! unit :=
+  let code := [
+    Bytecode.LdU32 42;
+    Bytecode.Pack (StructDefinitionIndex.Build_t 0);
+    Bytecode.MutBorrowLoc 0;
+    Bytecode.WriteRef
+  ] in
+  let module := make_module_with_local code (SignatureToken.Struct (StructHandleIndex.Build_t 0)) in
+  let module := add_simple_struct_with_abilities module AbilitySet.EMPTY in
+  let! fun_context := get_fun_context module in
+  assert_major_status
+    (verify module fun_context)
+    (fun status =>
+      match status with
+      | StatusCode.WRITEREF_WITHOUT_DROP_ABILITY => true
+      | _ => false
+      end
+    ).
+
+Goal test_write_ref_no_drop = return! tt.
+Proof. reflexivity. Qed.
+
+(*
+#[test]
+#[should_panic]
+fn test_write_ref_too_few_args() {
+    let code = vec![Bytecode::MutBorrowLoc(0), Bytecode::WriteRef];
+    let module = make_module_with_local(code, SignatureToken::U32);
+    let fun_context = get_fun_context(&module);
+    let _result = type_safety::verify(&module, &fun_context, &mut DummyMeter);
+}
+*)
+Definition test_write_ref_too_few_args : M!? _ unit :=
+  let code := [Bytecode.MutBorrowLoc 0; Bytecode.WriteRef] in
+  let module := make_module_with_local code SignatureToken.U32 in
+  let! fun_context := get_fun_context module in
+  verify module fun_context.
+
+Goal
+  exists (Error : Set) (error : Error),
+  test_write_ref_too_few_args = panic! error.
+Proof. repeat eexists. Qed.
+
+(*
+#[test]
+#[should_panic]
+fn test_write_ref_no_args() {
+    let code = vec![Bytecode::WriteRef];
+    let module = make_module_with_local(code, SignatureToken::U64);
+    let fun_context = get_fun_context(&module);
+    let _result = type_safety::verify(&module, &fun_context, &mut DummyMeter);
+}
+*)
+Definition test_write_ref_no_args : M!? _ unit :=
+  let code := [Bytecode.WriteRef] in
+  let module := make_module_with_local code SignatureToken.U64 in
+  let! fun_context := get_fun_context module in
+  verify module fun_context.
+
+Goal
+  exists (Error : Set) (error : Error),
+  test_write_ref_no_args = panic! error.
+Proof. repeat eexists. Qed.
+
+(*
+#[test]
+fn test_imm_borrow_field_correct_type() {
+    let code = vec![
+        Bytecode::ImmBorrowLoc(0),
+        Bytecode::ImmBorrowField(FieldHandleIndex(0)),
+    ];
+    let mut module = make_module_with_local(code, SignatureToken::Struct(StructHandleIndex(0)));
+    add_simple_struct(&mut module);
+    let fun_context = get_fun_context(&module);
+    let result = type_safety::verify(&module, &fun_context, &mut DummyMeter);
+    assert!(result.is_ok());
+}
+*)
+Definition test_imm_borrow_field_correct_type : M! unit :=
+  let code := [
+    Bytecode.ImmBorrowLoc 0;
+    Bytecode.ImmBorrowField (FieldHandleIndex.Build_t 0)
+  ] in
+  let module := make_module_with_local code (SignatureToken.Struct (StructHandleIndex.Build_t 0)) in
+  let module := add_simple_struct module in
+  let! fun_context := get_fun_context module in
+  let! result := verify module fun_context in
+  assert_is_ok result.
+
+Goal test_imm_borrow_field_correct_type = return! tt.
+Proof. reflexivity. Qed.
+
+(*
+#[test]
+fn test_imm_borrow_field_wrong_type() {
+    let code = vec![
+        Bytecode::LdTrue,
+        Bytecode::ImmBorrowField(FieldHandleIndex(0)),
+    ];
+    let mut module = make_module_with_local(code, SignatureToken::Struct(StructHandleIndex(0)));
+    add_simple_struct(&mut module);
+    let fun_context = get_fun_context(&module);
+    let result = type_safety::verify(&module, &fun_context, &mut DummyMeter);
+    assert_eq!(
+        result.unwrap_err().major_status(),
+        StatusCode::BORROWFIELD_TYPE_MISMATCH_ERROR
+    );
+}
+*)
+Definition test_imm_borrow_field_wrong_type : M! unit :=
+  let code := [
+    Bytecode.LdTrue;
+    Bytecode.ImmBorrowField (FieldHandleIndex.Build_t 0)
+  ] in
+  let module := make_module_with_local code (SignatureToken.Struct (StructHandleIndex.Build_t 0)) in
+  let module := add_simple_struct module in
+  let! fun_context := get_fun_context module in
+  assert_major_status
+    (verify module fun_context)
+    (fun status =>
+      match status with
+      | StatusCode.BORROWFIELD_TYPE_MISMATCH_ERROR => true
+      | _ => false
+      end
+    ).
+
+Goal test_imm_borrow_field_wrong_type = return! tt.
+Proof. reflexivity. Qed.
+
+(*
+#[test]
+fn test_imm_borrow_field_mismatched_types() {
+    let code = vec![
+        Bytecode::ImmBorrowLoc(0),
+        Bytecode::ImmBorrowField(FieldHandleIndex(0)),
+    ];
+    let mut module = make_module_with_local(code, SignatureToken::U64);
+    add_simple_struct(&mut module);
+    let fun_context = get_fun_context(&module);
+    let result = type_safety::verify(&module, &fun_context, &mut DummyMeter);
+    assert_eq!(
+        result.unwrap_err().major_status(),
+        StatusCode::BORROWFIELD_TYPE_MISMATCH_ERROR
+    );
+}
+*)
+Definition test_imm_borrow_field_mismatched_types : M! unit :=
+  let code := [
+    Bytecode.ImmBorrowLoc 0;
+    Bytecode.ImmBorrowField (FieldHandleIndex.Build_t 0)
+  ] in
+  let module := make_module_with_local code SignatureToken.U64 in
+  let module := add_simple_struct module in
+  let! fun_context := get_fun_context module in
+  assert_major_status
+    (verify module fun_context)
+    (fun status =>
+      match status with
+      | StatusCode.BORROWFIELD_TYPE_MISMATCH_ERROR => true
+      | _ => false
+      end
+    ).
+
+Goal test_imm_borrow_field_mismatched_types = return! tt.
+Proof. reflexivity. Qed.
+
+(*
+#[test]
+fn test_imm_borrow_field_bad_field() {
+    let code = vec![
+        Bytecode::ImmBorrowLoc(0),
+        Bytecode::ImmBorrowField(FieldHandleIndex(0)),
+    ];
+    let mut module = make_module_with_local(code, SignatureToken::Struct(StructHandleIndex(0)));
+    add_native_struct(&mut module);
+    let fun_context = get_fun_context(&module);
+    let result = type_safety::verify(&module, &fun_context, &mut DummyMeter);
+    assert_eq!(
+        result.unwrap_err().major_status(),
+        StatusCode::BORROWFIELD_BAD_FIELD_ERROR
+    );
+}
+*)
+Definition test_imm_borrow_field_bad_field : M! unit :=
+  let code := [
+    Bytecode.ImmBorrowLoc 0;
+    Bytecode.ImmBorrowField (FieldHandleIndex.Build_t 0)
+  ] in
+  let module := make_module_with_local code (SignatureToken.Struct (StructHandleIndex.Build_t 0)) in
+  let module := add_native_struct module in
+  let! fun_context := get_fun_context module in
+  assert_major_status
+    (verify module fun_context)
+    (fun status =>
+      match status with
+      | StatusCode.BORROWFIELD_BAD_FIELD_ERROR => true
+      | _ => false
+      end
+    ).
+
+Goal test_imm_borrow_field_bad_field = return! tt.
+Proof. reflexivity. Qed.
+
+(*
+#[test]
+#[should_panic]
+fn test_imm_borrow_field_no_arg() {
+    let code = vec![Bytecode::ImmBorrowField(FieldHandleIndex(0))];
+    let mut module = make_module_with_local(code, SignatureToken::Struct(StructHandleIndex(0)));
+    add_simple_struct(&mut module);
+    let fun_context = get_fun_context(&module);
+    let _result = type_safety::verify(&module, &fun_context, &mut DummyMeter);
+}
+*)
+Definition test_imm_borrow_field_no_arg : M!? _ unit :=
+  let code := [Bytecode.ImmBorrowField (FieldHandleIndex.Build_t 0)] in
+  let module := make_module_with_local code (SignatureToken.Struct (StructHandleIndex.Build_t 0)) in
+  let module := add_simple_struct module in
+  let! fun_context := get_fun_context module in
+  verify module fun_context.
+
+Goal
+  exists (Error : Set) (error : Error),
+  test_imm_borrow_field_no_arg = panic! error.
+Proof. repeat eexists. Qed.
+
+(*
+#[test]
+fn test_imm_borrow_field_generic_correct_type() {
+    let code = vec![
+        Bytecode::ImmBorrowLoc(0),
+        Bytecode::ImmBorrowFieldGeneric(FieldInstantiationIndex(0)),
+    ];
+    let signature = SignatureToken::StructInstantiation(Box::new((
+        StructHandleIndex(0),
+        vec![SignatureToken::U64],
+    )));
+    let mut module: CompiledModule = make_module_with_local(code, signature);
+    add_simple_struct_generic_with_abilities(
+        &mut module,
+        AbilitySet::PRIMITIVES,
+        SignatureToken::U64,
+    );
+    let fun_context = get_fun_context(&module);
+    let result = type_safety::verify(&module, &fun_context, &mut DummyMeter);
+    assert!(result.is_ok());
+}
+*)
+Definition test_imm_borrow_field_generic_correct_type : M! unit :=
+  let code := [
+    Bytecode.ImmBorrowLoc 0;
+    Bytecode.ImmBorrowFieldGeneric (FieldInstantiationIndex.Build_t 0)
+  ] in
+  let signature := SignatureToken.StructInstantiation (
+    StructHandleIndex.Build_t 0,
+    [SignatureToken.U64]
+  ) in
+  let module := make_module_with_local code signature in
+  let module := add_simple_struct_generic_with_abilities module AbilitySet.PRIMITIVES SignatureToken.U64 in
+  let! fun_context := get_fun_context module in
+  let! result := verify module fun_context in
+  assert_is_ok result.
+
+Goal test_imm_borrow_field_generic_correct_type = return! tt.
+Proof. reflexivity. Qed.
+
+(*
+#[test]
+fn test_imm_borrow_field_generic_wrong_type() {
+    let code = vec![
+        Bytecode::LdTrue,
+        Bytecode::ImmBorrowFieldGeneric(FieldInstantiationIndex(0)),
+    ];
+    let signature = SignatureToken::StructInstantiation(Box::new((
+        StructHandleIndex(0),
+        vec![SignatureToken::U64],
+    )));
+    let mut module = make_module_with_local(code, signature);
+    add_simple_struct_generic_with_abilities(
+        &mut module,
+        AbilitySet::PRIMITIVES,
+        SignatureToken::U64,
+    );
+    let fun_context = get_fun_context(&module);
+    let result = type_safety::verify(&module, &fun_context, &mut DummyMeter);
+    assert_eq!(
+        result.unwrap_err().major_status(),
+        StatusCode::BORROWFIELD_TYPE_MISMATCH_ERROR
+    );
+}
+*)
+Definition test_imm_borrow_field_generic_wrong_type : M! unit :=
+  let code := [
+    Bytecode.LdTrue;
+    Bytecode.ImmBorrowFieldGeneric (FieldInstantiationIndex.Build_t 0)
+  ] in
+  let signature := SignatureToken.StructInstantiation (
+    StructHandleIndex.Build_t 0,
+    [SignatureToken.U64]
+  ) in
+  let module := make_module_with_local code signature in
+  let module := add_simple_struct_generic_with_abilities module AbilitySet.PRIMITIVES SignatureToken.U64 in
+  let! fun_context := get_fun_context module in
+  assert_major_status
+    (verify module fun_context)
+    (fun status =>
+      match status with
+      | StatusCode.BORROWFIELD_TYPE_MISMATCH_ERROR => true
+      | _ => false
+      end
+    ).
+
+Goal test_imm_borrow_field_generic_wrong_type = return! tt.
+Proof. reflexivity. Qed.
+
+(*
+#[test]
+fn test_imm_borrow_field_generic_mismatched_types() {
+    let code = vec![
+        Bytecode::ImmBorrowLoc(0),
+        Bytecode::ImmBorrowFieldGeneric(FieldInstantiationIndex(0)),
+    ];
+    let mut module = make_module_with_local(code, SignatureToken::U64);
+    add_simple_struct_generic_with_abilities(
+        &mut module,
+        AbilitySet::PRIMITIVES,
+        SignatureToken::U64,
+    );
+    let fun_context = get_fun_context(&module);
+    let result = type_safety::verify(&module, &fun_context, &mut DummyMeter);
+    assert_eq!(
+        result.unwrap_err().major_status(),
+        StatusCode::BORROWFIELD_TYPE_MISMATCH_ERROR
+    );
+}
+*)
+Definition test_imm_borrow_field_generic_mismatched_types : M! unit :=
+  let code := [
+    Bytecode.ImmBorrowLoc 0;
+    Bytecode.ImmBorrowFieldGeneric (FieldInstantiationIndex.Build_t 0)
+  ] in
+  let module := make_module_with_local code SignatureToken.U64 in
+  let module := add_simple_struct_generic_with_abilities module AbilitySet.PRIMITIVES SignatureToken.U64 in
+  let! fun_context := get_fun_context module in
+  assert_major_status
+    (verify module fun_context)
+    (fun status =>
+      match status with
+      | StatusCode.BORROWFIELD_TYPE_MISMATCH_ERROR => true
+      | _ => false
+      end
+    ).
+
+Goal test_imm_borrow_field_generic_mismatched_types = return! tt.
+Proof. reflexivity. Qed.
+
+(*
+#[test]
+fn test_imm_borrow_field_generic_bad_field() {
+    let code = vec![
+        Bytecode::ImmBorrowLoc(0),
+        Bytecode::ImmBorrowFieldGeneric(FieldInstantiationIndex(0)),
+    ];
+    let signature = SignatureToken::StructInstantiation(Box::new((
+        StructHandleIndex(0),
+        vec![SignatureToken::U64],
+    )));
+    let mut module = make_module_with_local(code, signature);
+    add_native_struct_generic(&mut module, SignatureToken::U64);
+    let fun_context = get_fun_context(&module);
+    let result = type_safety::verify(&module, &fun_context, &mut DummyMeter);
+    assert_eq!(
+        result.unwrap_err().major_status(),
+        StatusCode::BORROWFIELD_BAD_FIELD_ERROR
+    );
+}
+*)
+Definition test_imm_borrow_field_generic_bad_field : M! unit :=
+  let code := [
+    Bytecode.ImmBorrowLoc 0;
+    Bytecode.ImmBorrowFieldGeneric (FieldInstantiationIndex.Build_t 0)
+  ] in
+  let signature := SignatureToken.StructInstantiation (
+    StructHandleIndex.Build_t 0,
+    [SignatureToken.U64]
+  ) in
+  let module := make_module_with_local code signature in
+  let module := add_native_struct_generic module SignatureToken.U64 in
+  let! fun_context := get_fun_context module in
+  assert_major_status
+    (verify module fun_context)
+    (fun status =>
+      match status with
+      | StatusCode.BORROWFIELD_BAD_FIELD_ERROR => true
+      | _ => false
+      end
+    ).
+
+Goal test_imm_borrow_field_generic_bad_field = return! tt.
+Proof. reflexivity. Qed.
+
+(*
+#[test]
+#[should_panic]
+fn test_imm_borrow_field_generic_no_arg() {
+    let code = vec![Bytecode::ImmBorrowFieldGeneric(FieldInstantiationIndex(0))];
+    let signature = SignatureToken::StructInstantiation(Box::new((
+        StructHandleIndex(0),
+        vec![SignatureToken::U64],
+    )));
+    let mut module = make_module_with_local(code, signature);
+    add_simple_struct_generic_with_abilities(
+        &mut module,
+        AbilitySet::PRIMITIVES,
+        SignatureToken::U64,
+    );
+    let fun_context = get_fun_context(&module);
+    let _result = type_safety::verify(&module, &fun_context, &mut DummyMeter);
+}
+*)
+Definition test_imm_borrow_field_generic_no_arg : M!? _ unit :=
+  let code := [Bytecode.ImmBorrowFieldGeneric (FieldInstantiationIndex.Build_t 0)] in
+  let signature := SignatureToken.StructInstantiation (
+    StructHandleIndex.Build_t 0,
+    [SignatureToken.U64]
+  ) in
+  let module := make_module_with_local code signature in
+  let module := add_simple_struct_generic_with_abilities module AbilitySet.PRIMITIVES SignatureToken.U64 in
+  let! fun_context := get_fun_context module in
+  verify module fun_context.
+
+Goal
+  exists (Error : Set) (error : Error),
+  test_imm_borrow_field_generic_no_arg = panic! error.
+Proof. repeat eexists. Qed.
+
+(*
+#[test]
+fn test_mut_borrow_field_correct_type() {
+    let code = vec![
+        Bytecode::MutBorrowLoc(0),
+        Bytecode::MutBorrowField(FieldHandleIndex(0)),
+    ];
+    let mut module = make_module_with_local(code, SignatureToken::Struct(StructHandleIndex(0)));
+    add_simple_struct(&mut module);
+    let fun_context = get_fun_context(&module);
+    let result = type_safety::verify(&module, &fun_context, &mut DummyMeter);
+    assert!(result.is_ok());
+}
+*)
+Definition test_mut_borrow_field_correct_type : M! unit :=
+  let code := [
+    Bytecode.MutBorrowLoc 0;
+    Bytecode.MutBorrowField (FieldHandleIndex.Build_t 0)
+  ] in
+  let module := make_module_with_local code (SignatureToken.Struct (StructHandleIndex.Build_t 0)) in
+  let module := add_simple_struct module in
+  let! fun_context := get_fun_context module in
+  let! result := verify module fun_context in
+  assert_is_ok result.
+
+Goal test_mut_borrow_field_correct_type = return! tt.
+Proof. reflexivity. Qed.
+
+(*
+#[test]
+fn test_mut_borrow_field_wrong_type() {
+    let code = vec![
+        Bytecode::LdTrue,
+        Bytecode::MutBorrowField(FieldHandleIndex(0)),
+    ];
+    let mut module = make_module_with_local(code, SignatureToken::Struct(StructHandleIndex(0)));
+    add_simple_struct(&mut module);
+    let fun_context = get_fun_context(&module);
+    let result = type_safety::verify(&module, &fun_context, &mut DummyMeter);
+    assert_eq!(
+        result.unwrap_err().major_status(),
+        StatusCode::BORROWFIELD_TYPE_MISMATCH_ERROR
+    );
+
+    let code = vec![
+        Bytecode::ImmBorrowLoc(0),
+        Bytecode::MutBorrowField(FieldHandleIndex(0)),
+    ];
+    let mut module = make_module_with_local(code, SignatureToken::Struct(StructHandleIndex(0)));
+    add_simple_struct(&mut module);
+    let fun_context = get_fun_context(&module);
+    let result = type_safety::verify(&module, &fun_context, &mut DummyMeter);
+    assert_eq!(
+        result.unwrap_err().major_status(),
+        StatusCode::BORROWFIELD_TYPE_MISMATCH_ERROR
+    );
+}
+*)
+Definition test_mut_borrow_field_wrong_type : M! unit :=
+  let code := [
+    Bytecode.LdTrue;
+    Bytecode.MutBorrowField (FieldHandleIndex.Build_t 0)
+  ] in
+  let module := make_module_with_local code (SignatureToken.Struct (StructHandleIndex.Build_t 0)) in
+  let module := add_simple_struct module in
+  let! fun_context := get_fun_context module in
+  do! assert_major_status
+    (verify module fun_context)
+    (fun status =>
+      match status with
+      | StatusCode.BORROWFIELD_TYPE_MISMATCH_ERROR => true
+      | _ => false
+      end
+    ) in
+  let code := [
+    Bytecode.ImmBorrowLoc 0;
+    Bytecode.MutBorrowField (FieldHandleIndex.Build_t 0)
+  ] in
+  let module := make_module_with_local code (SignatureToken.Struct (StructHandleIndex.Build_t 0)) in
+  let module := add_simple_struct module in
+  let! fun_context := get_fun_context module in
+  assert_major_status
+    (verify module fun_context)
+    (fun status =>
+      match status with
+      | StatusCode.BORROWFIELD_TYPE_MISMATCH_ERROR => true
+      | _ => false
+      end
+    ).
+
+Goal test_mut_borrow_field_wrong_type = return! tt.
+Proof. reflexivity. Qed.
+
+(*
+#[test]
+fn test_mut_borrow_field_mismatched_types() {
+    let code = vec![
+        Bytecode::MutBorrowLoc(0),
+        Bytecode::MutBorrowField(FieldHandleIndex(0)),
+    ];
+    let mut module = make_module_with_local(code, SignatureToken::U64);
+    add_simple_struct(&mut module);
+    let fun_context = get_fun_context(&module);
+    let result = type_safety::verify(&module, &fun_context, &mut DummyMeter);
+    assert_eq!(
+        result.unwrap_err().major_status(),
+        StatusCode::BORROWFIELD_TYPE_MISMATCH_ERROR
+    );
+}
+*)
+Definition test_mut_borrow_field_mismatched_types : M! unit :=
+  let code := [
+    Bytecode.MutBorrowLoc 0;
+    Bytecode.MutBorrowField (FieldHandleIndex.Build_t 0)
+  ] in
+  let module := make_module_with_local code SignatureToken.U64 in
+  let module := add_simple_struct module in
+  let! fun_context := get_fun_context module in
+  assert_major_status
+    (verify module fun_context)
+    (fun status =>
+      match status with
+      | StatusCode.BORROWFIELD_TYPE_MISMATCH_ERROR => true
+      | _ => false
+      end
+    ).
+
+Goal test_mut_borrow_field_mismatched_types = return! tt.
+Proof. reflexivity. Qed.
+
+(*
+#[test]
+fn test_mut_borrow_field_bad_field() {
+    let code = vec![
+        Bytecode::MutBorrowLoc(0),
+        Bytecode::MutBorrowField(FieldHandleIndex(0)),
+    ];
+    let mut module = make_module_with_local(code, SignatureToken::Struct(StructHandleIndex(0)));
+    add_native_struct(&mut module);
+    let fun_context = get_fun_context(&module);
+    let result = type_safety::verify(&module, &fun_context, &mut DummyMeter);
+    assert_eq!(
+        result.unwrap_err().major_status(),
+        StatusCode::BORROWFIELD_BAD_FIELD_ERROR
+    );
+}
+*)
+Definition test_mut_borrow_field_bad_field : M! unit :=
+  let code := [
+    Bytecode.MutBorrowLoc 0;
+    Bytecode.MutBorrowField (FieldHandleIndex.Build_t 0)
+  ] in
+  let module := make_module_with_local code (SignatureToken.Struct (StructHandleIndex.Build_t 0)) in
+  let module := add_native_struct module in
+  let! fun_context := get_fun_context module in
+  assert_major_status
+    (verify module fun_context)
+    (fun status =>
+      match status with
+      | StatusCode.BORROWFIELD_BAD_FIELD_ERROR => true
+      | _ => false
+      end
+    ).
+
+Goal test_mut_borrow_field_bad_field = return! tt.
+Proof. reflexivity. Qed.
+
+(*
+#[test]
+#[should_panic]
+fn test_mut_borrow_field_no_arg() {
+    let code = vec![Bytecode::MutBorrowField(FieldHandleIndex(0))];
+    let mut module = make_module_with_local(code, SignatureToken::Struct(StructHandleIndex(0)));
+    add_simple_struct(&mut module);
+    let fun_context = get_fun_context(&module);
+    let _result = type_safety::verify(&module, &fun_context, &mut DummyMeter);
+}
+*)
+Definition test_mut_borrow_field_no_arg : M!? _ unit :=
+  let code := [Bytecode.MutBorrowField (FieldHandleIndex.Build_t 0)] in
+  let module := make_module_with_local code (SignatureToken.Struct (StructHandleIndex.Build_t 0)) in
+  let module := add_simple_struct module in
+  let! fun_context := get_fun_context module in
+  verify module fun_context.
+
+Goal
+  exists (Error : Set) (error : Error),
+  test_mut_borrow_field_no_arg = panic! error.
+Proof. repeat eexists. Qed.
+
+(*
+#[test]
+fn test_mut_borrow_field_generic_correct_type() {
+    let code = vec![
+        Bytecode::MutBorrowLoc(0),
+        Bytecode::MutBorrowFieldGeneric(FieldInstantiationIndex(0)),
+    ];
+    let signature = SignatureToken::StructInstantiation(Box::new((
+        StructHandleIndex(0),
+        vec![SignatureToken::U64],
+    )));
+    let mut module = make_module_with_local(code, signature);
+    add_simple_struct_generic_with_abilities(
+        &mut module,
+        AbilitySet::PRIMITIVES,
+        SignatureToken::U64,
+    );
+    let fun_context = get_fun_context(&module);
+    let result = type_safety::verify(&module, &fun_context, &mut DummyMeter);
+    assert!(result.is_ok());
+}
+*)
+Definition test_mut_borrow_field_generic_correct_type : M! unit :=
+  let code := [
+    Bytecode.MutBorrowLoc 0;
+    Bytecode.MutBorrowFieldGeneric (FieldInstantiationIndex.Build_t 0)
+  ] in
+  let signature := SignatureToken.StructInstantiation (
+    StructHandleIndex.Build_t 0,
+    [SignatureToken.U64]
+  ) in
+  let module := make_module_with_local code signature in
+  let module := add_simple_struct_generic_with_abilities module AbilitySet.PRIMITIVES SignatureToken.U64 in
+  let! fun_context := get_fun_context module in
+  let! result := verify module fun_context in
+  assert_is_ok result.
+
+Goal test_mut_borrow_field_generic_correct_type = return! tt.
+Proof. reflexivity. Qed.
+
+(*
+#[test]
+fn test_mut_borrow_field_generic_wrong_type() {
+    let code = vec![
+        Bytecode::LdTrue,
+        Bytecode::MutBorrowFieldGeneric(FieldInstantiationIndex(0)),
+    ];
+    let signature = SignatureToken::StructInstantiation(Box::new((
+        StructHandleIndex(0),
+        vec![SignatureToken::U64],
+    )));
+    let mut module = make_module_with_local(code, signature);
+    add_simple_struct_generic_with_abilities(
+        &mut module,
+        AbilitySet::PRIMITIVES,
+        SignatureToken::U64,
+    );
+    let fun_context = get_fun_context(&module);
+    let result = type_safety::verify(&module, &fun_context, &mut DummyMeter);
+    assert_eq!(
+        result.unwrap_err().major_status(),
+        StatusCode::BORROWFIELD_TYPE_MISMATCH_ERROR
+    );
+
+    let code = vec![
+        Bytecode::ImmBorrowLoc(0),
+        Bytecode::MutBorrowFieldGeneric(FieldInstantiationIndex(0)),
+    ];
+    let signature = SignatureToken::StructInstantiation(Box::new((
+        StructHandleIndex(0),
+        vec![SignatureToken::U64],
+    )));
+    let mut module = make_module_with_local(code, signature);
+    add_simple_struct_generic_with_abilities(
+        &mut module,
+        AbilitySet::PRIMITIVES,
+        SignatureToken::U64,
+    );
+    let fun_context = get_fun_context(&module);
+    let result = type_safety::verify(&module, &fun_context, &mut DummyMeter);
+    assert_eq!(
+        result.unwrap_err().major_status(),
+        StatusCode::BORROWFIELD_TYPE_MISMATCH_ERROR
+    );
+}
+*)
+Definition test_mut_borrow_field_generic_wrong_type : M! unit :=
+  let code := [
+    Bytecode.LdTrue;
+    Bytecode.MutBorrowFieldGeneric (FieldInstantiationIndex.Build_t 0)
+  ] in
+  let signature := SignatureToken.StructInstantiation (
+    StructHandleIndex.Build_t 0,
+    [SignatureToken.U64]
+  ) in
+  let module := make_module_with_local code signature in
+  let module := add_simple_struct_generic_with_abilities module AbilitySet.PRIMITIVES SignatureToken.U64 in
+  let! fun_context := get_fun_context module in
+  do! assert_major_status
+    (verify module fun_context)
+    (fun status =>
+      match status with
+      | StatusCode.BORROWFIELD_TYPE_MISMATCH_ERROR => true
+      | _ => false
+      end
+    ) in
+  let code := [
+    Bytecode.ImmBorrowLoc 0;
+    Bytecode.MutBorrowFieldGeneric (FieldInstantiationIndex.Build_t 0)
+  ] in
+  let signature := SignatureToken.StructInstantiation (
+    StructHandleIndex.Build_t 0,
+    [SignatureToken.U64]
+  ) in
+  let module := make_module_with_local code signature in
+  let module := add_simple_struct_generic_with_abilities module AbilitySet.PRIMITIVES SignatureToken.U64 in
+  let! fun_context := get_fun_context module in
+  assert_major_status
+    (verify module fun_context)
+    (fun status =>
+      match status with
+      | StatusCode.BORROWFIELD_TYPE_MISMATCH_ERROR => true
+      | _ => false
+      end
+    ).
+
+Goal test_mut_borrow_field_generic_wrong_type = return! tt.
+Proof. reflexivity. Qed.
+
+(*
+#[test]
+fn test_mut_borrow_field_generic_mismatched_types() {
+    let code = vec![
+        Bytecode::MutBorrowLoc(0),
+        Bytecode::MutBorrowFieldGeneric(FieldInstantiationIndex(0)),
+    ];
+    let mut module: CompiledModule = make_module_with_local(code, SignatureToken::U64);
+    add_simple_struct_generic_with_abilities(
+        &mut module,
+        AbilitySet::PRIMITIVES,
+        SignatureToken::U64,
+    );
+    let fun_context = get_fun_context(&module);
+    let result = type_safety::verify(&module, &fun_context, &mut DummyMeter);
+    assert_eq!(
+        result.unwrap_err().major_status(),
+        StatusCode::BORROWFIELD_TYPE_MISMATCH_ERROR
+    );
+}
+*)
+Definition test_mut_borrow_field_generic_mismatched_types : M! unit :=
+  let code := [
+    Bytecode.MutBorrowLoc 0;
+    Bytecode.MutBorrowFieldGeneric (FieldInstantiationIndex.Build_t 0)
+  ] in
+  let module := make_module_with_local code SignatureToken.U64 in
+  let module := add_simple_struct_generic_with_abilities module AbilitySet.PRIMITIVES SignatureToken.U64 in
+  let! fun_context := get_fun_context module in
+  assert_major_status
+    (verify module fun_context)
+    (fun status =>
+      match status with
+      | StatusCode.BORROWFIELD_TYPE_MISMATCH_ERROR => true
+      | _ => false
+      end
+    ).
+
+Goal test_mut_borrow_field_generic_mismatched_types = return! tt.
+Proof. reflexivity. Qed.
+
+(*
+#[test]
+fn test_mut_borrow_field_generic_bad_field() {
+    let code = vec![
+        Bytecode::MutBorrowLoc(0),
+        Bytecode::MutBorrowFieldGeneric(FieldInstantiationIndex(0)),
+    ];
+    let signature = SignatureToken::StructInstantiation(Box::new((
+        StructHandleIndex(0),
+        vec![SignatureToken::U64],
+    )));
+    let mut module = make_module_with_local(code, signature);
+    add_native_struct_generic(&mut module, SignatureToken::U64);
+    let fun_context = get_fun_context(&module);
+    let result = type_safety::verify(&module, &fun_context, &mut DummyMeter);
+    assert_eq!(
+        result.unwrap_err().major_status(),
+        StatusCode::BORROWFIELD_BAD_FIELD_ERROR
+    );
+}
+*)
+Definition test_mut_borrow_field_generic_bad_field : M! unit :=
+  let code := [
+    Bytecode.MutBorrowLoc 0;
+    Bytecode.MutBorrowFieldGeneric (FieldInstantiationIndex.Build_t 0)
+  ] in
+  let signature := SignatureToken.StructInstantiation (
+    StructHandleIndex.Build_t 0,
+    [SignatureToken.U64]
+  ) in
+  let module := make_module_with_local code signature in
+  let module := add_native_struct_generic module SignatureToken.U64 in
+  let! fun_context := get_fun_context module in
+  assert_major_status
+    (verify module fun_context)
+    (fun status =>
+      match status with
+      | StatusCode.BORROWFIELD_BAD_FIELD_ERROR => true
+      | _ => false
+      end
+    ).
+
+Goal test_mut_borrow_field_generic_bad_field = return! tt.
+Proof. reflexivity. Qed.
+
+(*
+#[test]
+#[should_panic]
+fn test_mut_borrow_field_generic_no_arg() {
+    let code = vec![Bytecode::MutBorrowFieldGeneric(FieldInstantiationIndex(0))];
+    let signature = SignatureToken::StructInstantiation(Box::new((
+        StructHandleIndex(0),
+        vec![SignatureToken::U64],
+    )));
+    let mut module = make_module_with_local(code, signature);
+    add_simple_struct_generic_with_abilities(
+        &mut module,
+        AbilitySet::PRIMITIVES,
+        SignatureToken::U64,
+    );
+    let fun_context = get_fun_context(&module);
+    let _result = type_safety::verify(&module, &fun_context, &mut DummyMeter);
+}
+*)
+Definition test_mut_borrow_field_generic_no_arg : M!? _ unit :=
+  let code := [Bytecode.MutBorrowFieldGeneric (FieldInstantiationIndex.Build_t 0)] in
+  let signature := SignatureToken.StructInstantiation (
+    StructHandleIndex.Build_t 0,
+    [SignatureToken.U64]
+  ) in
+  let module := make_module_with_local code signature in
+  let module := add_simple_struct_generic_with_abilities module AbilitySet.PRIMITIVES SignatureToken.U64 in
+  let! fun_context := get_fun_context module in
+  verify module fun_context.
+
+Goal
+  exists (Error : Set) (error : Error),
+  test_mut_borrow_field_generic_no_arg = panic! error.
+Proof. repeat eexists. Qed.
+
+(*
+#[test]
+fn test_ret_correct_type() {
+    let code = vec![Bytecode::LdU32(42), Bytecode::Ret];
+    let module = make_module_with_ret(code, SignatureToken::U32);
+    let fun_context = get_fun_context(&module);
+    let result = type_safety::verify(&module, &fun_context, &mut DummyMeter);
+    assert!(result.is_ok());
+}
+*)
+Definition test_ret_correct_type : M! unit :=
+  let code := [
+    Bytecode.LdU32 42;
+    Bytecode.Ret
+  ] in
+  let module := make_module_with_ret code SignatureToken.U32 in
+  let! fun_context := get_fun_context module in
+  let! result := verify module fun_context in
+  assert_is_ok result.
+
+Goal test_ret_correct_type = return! tt.
+Proof. reflexivity. Qed.
+
+(*
+#[test]
+fn test_ret_wrong_type() {
+    let code = vec![Bytecode::LdU64(42), Bytecode::Ret];
+    let module = make_module_with_ret(code, SignatureToken::U32);
+    let fun_context = get_fun_context(&module);
+    let result = type_safety::verify(&module, &fun_context, &mut DummyMeter);
+    assert_eq!(
+        result.unwrap_err().major_status(),
+        StatusCode::RET_TYPE_MISMATCH_ERROR
+    );
+}
+*)
+Definition test_ret_wrong_type : M! unit :=
+  let code := [
+    Bytecode.LdU64 42;
+    Bytecode.Ret
+  ] in
+  let module := make_module_with_ret code SignatureToken.U32 in
+  let! fun_context := get_fun_context module in
+  assert_major_status
+    (verify module fun_context)
+    (fun status =>
+      match status with
+      | StatusCode.RET_TYPE_MISMATCH_ERROR => true
+      | _ => false
+      end
+    ).
+
+Goal test_ret_wrong_type = return! tt.
+Proof. reflexivity. Qed.
+
+(*
+#[test]
+#[should_panic]
+fn test_ret_no_arg() {
+    let code = vec![Bytecode::Ret];
+    let module = make_module_with_ret(code, SignatureToken::U32);
+    let fun_context = get_fun_context(&module);
+    let _result = type_safety::verify(&module, &fun_context, &mut DummyMeter);
+}
+*)
+Definition test_ret_no_arg : M!? _ unit :=
+  let code := [Bytecode.Ret] in
+  let module := make_module_with_ret code SignatureToken.U32 in
+  let! fun_context := get_fun_context module in
+  verify module fun_context.
+
+Goal
+  exists (Error : Set) (error : Error),
+  test_ret_no_arg = panic! error.
+Proof. repeat eexists. Qed.
+
+(*
+#[test]
+fn test_call_correct_types() {
+    let code = vec![
+        Bytecode::LdU64(42),
+        Bytecode::LdTrue,
+        Bytecode::Call(FunctionHandleIndex(1)),
+    ];
+    let parameters = Signature(vec![SignatureToken::U64, SignatureToken::Bool]);
+    let mut module = make_module(code);
+    add_function_with_parameters(&mut module, parameters);
+    let fun_context = get_fun_context(&module);
+    let result = type_safety::verify(&module, &fun_context, &mut DummyMeter);
+    assert!(result.is_ok());
+}
+*)
+Definition test_call_correct_types : M! unit :=
+  let code := [
+    Bytecode.LdU64 42;
+    Bytecode.LdTrue;
+    Bytecode.Call (FunctionHandleIndex.Build_t 1)
+  ] in
+  let parameters := Signature.Build_t [SignatureToken.U64; SignatureToken.Bool] in
+  let module := make_module code in
+  let module := add_function_with_parameters module parameters in
+  let! fun_context := get_fun_context module in
+  let! result := verify module fun_context in
+  assert_is_ok result.
+
+Goal test_call_correct_types = return! tt.
+Proof. reflexivity. Qed.
+
+(*
+#[test]
+fn test_call_wrong_types() {
+    let code = vec![
+        Bytecode::LdTrue,
+        Bytecode::LdU64(42),
+        Bytecode::Call(FunctionHandleIndex(1)),
+    ];
+    let parameters = Signature(vec![SignatureToken::U64, SignatureToken::Bool]);
+    let mut module = make_module(code);
+    add_function_with_parameters(&mut module, parameters);
+    let fun_context = get_fun_context(&module);
+    let result = type_safety::verify(&module, &fun_context, &mut DummyMeter);
+    assert_eq!(
+        result.unwrap_err().major_status(),
+        StatusCode::CALL_TYPE_MISMATCH_ERROR
+    );
+}
+*)
+Definition test_call_wrong_types : M! unit :=
+  let code := [
+    Bytecode.LdTrue;
+    Bytecode.LdU64 42;
+    Bytecode.Call (FunctionHandleIndex.Build_t 1)
+  ] in
+  let parameters := Signature.Build_t [SignatureToken.U64; SignatureToken.Bool] in
+  let module := make_module code in
+  let module := add_function_with_parameters module parameters in
+  let! fun_context := get_fun_context module in
+  assert_major_status
+    (verify module fun_context)
+    (fun status =>
+      match status with
+      | StatusCode.CALL_TYPE_MISMATCH_ERROR => true
+      | _ => false
+      end
+    ).
+
+Goal test_call_wrong_types = return! tt.
+Proof. reflexivity. Qed.
+
+(*
+#[test]
+#[should_panic]
+fn test_call_too_few_args() {
+    let code = vec![Bytecode::LdTrue, Bytecode::Call(FunctionHandleIndex(1))];
+    let parameters = Signature(vec![SignatureToken::U64, SignatureToken::Bool]);
+    let mut module = make_module(code);
+    add_function_with_parameters(&mut module, parameters);
+    let fun_context = get_fun_context(&module);
+    let _result = type_safety::verify(&module, &fun_context, &mut DummyMeter);
+}
+*)
+Definition test_call_too_few_args : M!? _ unit :=
+  let code := [Bytecode.LdTrue; Bytecode.Call (FunctionHandleIndex.Build_t 1)] in
+  let parameters := Signature.Build_t [SignatureToken.U64; SignatureToken.Bool] in
+  let module := make_module code in
+  let module := add_function_with_parameters module parameters in
+  let! fun_context := get_fun_context module in
+  verify module fun_context.
+
+Goal
+  exists (Error : Set) (error : Error),
+  test_call_too_few_args = panic! error.
+Proof. repeat eexists. Qed.
+
+(*
+#[test]
+fn test_call_generic_correct_types() {
+    let code = vec![
+        Bytecode::LdU32(42),
+        Bytecode::CallGeneric(FunctionInstantiationIndex(0)),
+    ];
+    let mut module = make_module(code);
+    add_generic_function_with_parameters(&mut module, SignatureToken::U32);
+    let fun_context = get_fun_context(&module);
+    let result = type_safety::verify(&module, &fun_context, &mut DummyMeter);
+    assert!(result.is_ok());
+
+    let code = vec![
+        Bytecode::LdU64(51),
+        Bytecode::CallGeneric(FunctionInstantiationIndex(0)),
+    ];
+    let mut module = make_module(code);
+    add_generic_function_with_parameters(&mut module, SignatureToken::U64);
+    let fun_context = get_fun_context(&module);
+    let result = type_safety::verify(&module, &fun_context, &mut DummyMeter);
+    assert!(result.is_ok());
+}
+*)
+Definition test_call_generic_correct_types : M! unit :=
+  let code := [
+    Bytecode.LdU32 42;
+    Bytecode.CallGeneric (FunctionInstantiationIndex.Build_t 0)
+  ] in
+  let module := make_module code in
+  let module := add_generic_function_with_parameters module SignatureToken.U32 in
+  let! fun_context := get_fun_context module in
+  let! result := verify module fun_context in
+  do! assert_is_ok result in
+  let code := [
+    Bytecode.LdU64 51;
+    Bytecode.CallGeneric (FunctionInstantiationIndex.Build_t 0)
+  ] in
+  let module := make_module code in
+  let module := add_generic_function_with_parameters module SignatureToken.U64 in
+  let! fun_context := get_fun_context module in
+  let! result := verify module fun_context in
+  assert_is_ok result.
+
+Goal test_call_generic_correct_types = return! tt.
+Proof. reflexivity. Qed.
+
+(*
+#[test]
+fn test_call_generic_wrong_types() {
+    let code = vec![
+        Bytecode::LdTrue,
+        Bytecode::CallGeneric(FunctionInstantiationIndex(0)),
+    ];
+    let mut module = make_module(code);
+    add_generic_function_with_parameters(&mut module, SignatureToken::U32);
+    let fun_context = get_fun_context(&module);
+    let result = type_safety::verify(&module, &fun_context, &mut DummyMeter);
+    assert_eq!(
+        result.unwrap_err().major_status(),
+        StatusCode::CALL_TYPE_MISMATCH_ERROR
+    );
+}
+*)
+Definition test_call_generic_wrong_types : M! unit :=
+  let code := [
+    Bytecode.LdTrue;
+    Bytecode.CallGeneric (FunctionInstantiationIndex.Build_t 0)
+  ] in
+  let module := make_module code in
+  let module := add_generic_function_with_parameters module SignatureToken.U32 in
+  let! fun_context := get_fun_context module in
+  assert_major_status
+    (verify module fun_context)
+    (fun status =>
+      match status with
+      | StatusCode.CALL_TYPE_MISMATCH_ERROR => true
+      | _ => false
+      end
+    ).
+
+Goal test_call_generic_wrong_types = return! tt.
+Proof. reflexivity. Qed.
+
+(*
+#[test]
+#[should_panic]
+fn test_call_generic_too_few_args() {
+    let code = vec![Bytecode::CallGeneric(FunctionInstantiationIndex(0))];
+    let mut module = make_module(code);
+    add_generic_function_with_parameters(&mut module, SignatureToken::U32);
+    let fun_context = get_fun_context(&module);
+    let _result = type_safety::verify(&module, &fun_context, &mut DummyMeter);
+}
+*)
+Definition test_call_generic_too_few_args : M!? _ unit :=
+  let code := [Bytecode.CallGeneric (FunctionInstantiationIndex.Build_t 0)] in
+  let module := make_module code in
+  let module := add_generic_function_with_parameters module SignatureToken.U32 in
+  let! fun_context := get_fun_context module in
+  verify module fun_context.
+
+Goal
+  exists (Error : Set) (error : Error),
+  test_call_generic_too_few_args = panic! error.
+Proof. repeat eexists. Qed.
+
+(*
+#[test]
+fn test_vec_pack_correct_type() {
+    let code = vec![
+        Bytecode::LdU32(33),
+        Bytecode::LdU32(42),
+        Bytecode::LdU32(51),
+        Bytecode::VecPack(SignatureIndex(1), 3),
+    ];
+    let module = make_module(code);
+    let fun_context = get_fun_context(&module);
+    let result = type_safety::verify(&module, &fun_context, &mut DummyMeter);
+    assert!(result.is_ok());
+}
+*)
+Definition test_vec_pack_correct_type : M! unit :=
+  let code := [
+    Bytecode.LdU32 33;
+    Bytecode.LdU32 42;
+    Bytecode.LdU32 51;
+    Bytecode.VecPack (SignatureIndex.Build_t 1) 3
+  ] in
+  let module := make_module code in
+  let! fun_context := get_fun_context module in
+  let! result := verify module fun_context in
+  assert_is_ok result.
+
+Goal test_vec_pack_correct_type = return! tt.
+Proof. reflexivity. Qed.
+
+(*
+#[test]
+fn test_vec_pack_wrong_type() {
+    let code = vec![
+        Bytecode::LdU32(33),
+        Bytecode::LdU64(42),
+        Bytecode::LdU32(51),
+        Bytecode::VecPack(SignatureIndex(1), 3),
+    ];
+    let module = make_module(code);
+    let fun_context = get_fun_context(&module);
+    let result = type_safety::verify(&module, &fun_context, &mut DummyMeter);
+    assert_eq!(
+        result.unwrap_err().major_status(),
+        StatusCode::TYPE_MISMATCH
+    );
+}
+*)
+Definition test_vec_pack_wrong_type : M! unit :=
+  let code := [
+    Bytecode.LdU32 33;
+    Bytecode.LdU64 42;
+    Bytecode.LdU32 51;
+    Bytecode.VecPack (SignatureIndex.Build_t 1) 3
+  ] in
+  let module := make_module code in
+  let! fun_context := get_fun_context module in
+  assert_major_status
+    (verify module fun_context)
+    (fun status =>
+      match status with
+      | StatusCode.TYPE_MISMATCH => true
+      | _ => false
+      end
+    ).
+
+Goal test_vec_pack_wrong_type = return! tt.
+Proof. reflexivity. Qed.
+
+(*
+#[test]
+fn test_vec_pack_too_few_args() {
+    let code = vec![
+        Bytecode::LdU32(33),
+        Bytecode::LdU32(51),
+        Bytecode::VecPack(SignatureIndex(1), 3),
+    ];
+    let module = make_module(code);
+    let fun_context = get_fun_context(&module);
+    let result = type_safety::verify(&module, &fun_context, &mut DummyMeter);
+    assert_eq!(
+        result.unwrap_err().major_status(),
+        StatusCode::TYPE_MISMATCH
+    );
+}
+*)
+Definition test_vec_pack_too_few_args : M! unit :=
+  let code := [
+    Bytecode.LdU32 33;
+    Bytecode.LdU32 51;
+    Bytecode.VecPack (SignatureIndex.Build_t 1) 3
+  ] in
+  let module := make_module code in
+  let! fun_context := get_fun_context module in
+  assert_major_status
+    (verify module fun_context)
+    (fun status =>
+      match status with
+      | StatusCode.TYPE_MISMATCH => true
+      | _ => false
+      end
+    ).
+
+Goal test_vec_pack_too_few_args = return! tt.
+Proof. reflexivity. Qed.
+
+(*
+#[test]
+fn test_vec_unpack_correct_type() {
+    let code = vec![
+        Bytecode::LdU32(33),
+        Bytecode::LdU32(42),
+        Bytecode::LdU32(51),
+        Bytecode::VecPack(SignatureIndex(1), 3),
+        Bytecode::VecUnpack(SignatureIndex(1), 3),
+    ];
+    let module = make_module(code);
+    let fun_context = get_fun_context(&module);
+    let result = type_safety::verify(&module, &fun_context, &mut DummyMeter);
+    assert!(result.is_ok());
+}
+*)
+Definition test_vec_unpack_correct_type : M! unit :=
+  let code := [
+    Bytecode.LdU32 33;
+    Bytecode.LdU32 42;
+    Bytecode.LdU32 51;
+    Bytecode.VecPack (SignatureIndex.Build_t 1) 3;
+    Bytecode.VecUnpack (SignatureIndex.Build_t 1) 3
+  ] in
+  let module := make_module code in
+  let! fun_context := get_fun_context module in
+  let! result := verify module fun_context in
+  assert_is_ok result.
+
+Goal test_vec_unpack_correct_type = return! tt.
+Proof. reflexivity. Qed.
+
+(*
+#[test]
+fn test_vec_unpack_wrong_type() {
+    let code = vec![
+        Bytecode::LdU32(33),
+        Bytecode::VecUnpack(SignatureIndex(1), 3),
+    ];
+    let module = make_module(code);
+    let fun_context = get_fun_context(&module);
+    let result = type_safety::verify(&module, &fun_context, &mut DummyMeter);
+    assert_eq!(
+        result.unwrap_err().major_status(),
+        StatusCode::TYPE_MISMATCH
+    );
+
+    let code = vec![
+        Bytecode::LdU32(33),
+        Bytecode::LdU32(42),
+        Bytecode::LdU64(51),
+        Bytecode::VecPack(SignatureIndex(1), 3),
+        Bytecode::VecUnpack(SignatureIndex(2), 3),
+    ];
+    let mut module = make_module(code);
+    module.signatures.push(Signature(vec![SignatureToken::U64]));
+    let fun_context = get_fun_context(&module);
+    let result = type_safety::verify(&module, &fun_context, &mut DummyMeter);
+    assert_eq!(
+        result.unwrap_err().major_status(),
+        StatusCode::TYPE_MISMATCH
+    );
+}
+*)
+Definition test_vec_unpack_wrong_type : M! unit :=
+  let code := [
+    Bytecode.LdU32 33;
+    Bytecode.VecUnpack (SignatureIndex.Build_t 1) 3
+  ] in
+  let module := make_module code in
+  let! fun_context := get_fun_context module in
+  do! assert_major_status
+    (verify module fun_context)
+    (fun status =>
+      match status with
+      | StatusCode.TYPE_MISMATCH => true
+      | _ => false
+      end
+    ) in
+  let code := [
+    Bytecode.LdU32 33;
+    Bytecode.LdU32 42;
+    Bytecode.LdU64 51;
+    Bytecode.VecPack (SignatureIndex.Build_t 1) 3;
+    Bytecode.VecUnpack (SignatureIndex.Build_t 2) 3
+  ] in
+  let module := make_module code in
+  let module := module <|
+    CompiledModule.signatures :=
+      module.(CompiledModule.signatures) ++ [Signature.Build_t [SignatureToken.U64]]
+  |> in
+  let! fun_context := get_fun_context module in
+  assert_major_status
+    (verify module fun_context)
+    (fun status =>
+      match status with
+      | StatusCode.TYPE_MISMATCH => true
+      | _ => false
+      end
+    ).
+
+Goal test_vec_unpack_wrong_type = return! tt.
+Proof. reflexivity. Qed.
+
+(*
+#[test]
+fn test_vec_unpack_too_few_elements() {
+    let code = vec![
+        Bytecode::LdU32(33),
+        Bytecode::LdU32(42),
+        Bytecode::LdU32(51),
+        Bytecode::VecPack(SignatureIndex(1), 3),
+        Bytecode::VecUnpack(SignatureIndex(1), 100500),
+    ];
+    let module = make_module(code);
+    let fun_context = get_fun_context(&module);
+    let result = type_safety::verify(&module, &fun_context, &mut DummyMeter);
+    assert!(result.is_ok());
+}
+*)
+Definition test_vec_unpack_too_few_elements : M! unit :=
+  let code := [
+    Bytecode.LdU32 33;
+    Bytecode.LdU32 42;
+    Bytecode.LdU32 51;
+    Bytecode.VecPack (SignatureIndex.Build_t 1) 3;
+    Bytecode.VecUnpack (SignatureIndex.Build_t 1) 100500
+  ] in
+  let module := make_module code in
+  let! fun_context := get_fun_context module in
+  let! result := verify module fun_context in
+  assert_is_ok result.
+
+Goal test_vec_unpack_too_few_elements = return! tt.
+Proof. reflexivity. Qed.
+
+(*
+#[test]
+#[should_panic]
+fn test_vec_unpack_no_arg() {
+    let code = vec![Bytecode::VecUnpack(SignatureIndex(1), 3)];
+    let module = make_module(code);
+    let fun_context = get_fun_context(&module);
+    let _result = type_safety::verify(&module, &fun_context, &mut DummyMeter);
+}
+*)
+Definition test_vec_unpack_no_arg : M!? _ unit :=
+  let code := [Bytecode.VecUnpack (SignatureIndex.Build_t 1) 3] in
+  let module := make_module code in
+  let! fun_context := get_fun_context module in
+  verify module fun_context.
+
+Goal
+  exists (Error : Set) (error : Error),
+  test_vec_unpack_no_arg = panic! error.
+Proof. repeat eexists. Qed.
+
+(*
+#[test]
+fn test_vec_len_correct_type() {
+    let code = vec![
+        Bytecode::ImmBorrowLoc(0),
+        Bytecode::VecLen(SignatureIndex(3)),
+    ];
+    let mut module =
+        make_module_with_local(code, SignatureToken::Vector(Box::new(SignatureToken::U32)));
+    module.signatures.push(Signature(vec![SignatureToken::U32]));
+    let fun_context = get_fun_context(&module);
+    let result = type_safety::verify(&module, &fun_context, &mut DummyMeter);
+    assert!(result.is_ok());
+}
+*)
+Definition test_vec_len_correct_type : M! unit :=
+  let code := [
+    Bytecode.ImmBorrowLoc 0;
+    Bytecode.VecLen (SignatureIndex.Build_t 3)
+  ] in
+  let module := make_module_with_local code (SignatureToken.Vector SignatureToken.U32) in
+  let module := module <|
+    CompiledModule.signatures :=
+      module.(CompiledModule.signatures) ++ [Signature.Build_t [SignatureToken.U32]]
+  |> in
+  let! fun_context := get_fun_context module in
+  let! result := verify module fun_context in
+  assert_is_ok result.
+
+Goal test_vec_len_correct_type = return! tt.
+Proof. reflexivity. Qed.
+
+(*
+#[test]
+fn test_vec_len_type_mismatch() {
+    let code = vec![
+        Bytecode::ImmBorrowLoc(0),
+        Bytecode::VecLen(SignatureIndex(3)),
+    ];
+    let mut module =
+        make_module_with_local(code, SignatureToken::Vector(Box::new(SignatureToken::U32)));
+    module.signatures.push(Signature(vec![SignatureToken::U64]));
+    let fun_context = get_fun_context(&module);
+    let result = type_safety::verify(&module, &fun_context, &mut DummyMeter);
+    assert_eq!(
+        result.unwrap_err().major_status(),
+        StatusCode::TYPE_MISMATCH
+    );
+}
+*)
+Definition test_vec_len_type_mismatch : M! unit :=
+  let code := [
+    Bytecode.ImmBorrowLoc 0;
+    Bytecode.VecLen (SignatureIndex.Build_t 3)
+  ] in
+  let module := make_module_with_local code (SignatureToken.Vector SignatureToken.U32) in
+  let module := module <|
+    CompiledModule.signatures :=
+      module.(CompiledModule.signatures) ++ [Signature.Build_t [SignatureToken.U64]]
+  |> in
+  let! fun_context := get_fun_context module in
+  assert_major_status
+    (verify module fun_context)
+    (fun status =>
+      match status with
+      | StatusCode.TYPE_MISMATCH => true
+      | _ => false
+      end
+    ).
+
+Goal test_vec_len_type_mismatch = return! tt.
+Proof. reflexivity. Qed.
+
+(*
+#[test]
+fn test_vec_len_wrong_type() {
+    let code = vec![Bytecode::LdU32(42), Bytecode::VecLen(SignatureIndex(3))];
+    let mut module =
+        make_module_with_local(code, SignatureToken::Vector(Box::new(SignatureToken::U32)));
+    module.signatures.push(Signature(vec![SignatureToken::U32]));
+    let fun_context = get_fun_context(&module);
+    let result = type_safety::verify(&module, &fun_context, &mut DummyMeter);
+    assert_eq!(
+        result.unwrap_err().major_status(),
+        StatusCode::TYPE_MISMATCH
+    );
+}
+*)
+Definition test_vec_len_wrong_type : M! unit :=
+  let code := [
+    Bytecode.LdU32 42;
+    Bytecode.VecLen (SignatureIndex.Build_t 3)
+  ] in
+  let module := make_module_with_local code (SignatureToken.Vector SignatureToken.U32) in
+  let module := module <|
+    CompiledModule.signatures :=
+      module.(CompiledModule.signatures) ++ [Signature.Build_t [SignatureToken.U32]]
+  |> in
+  let! fun_context := get_fun_context module in
+  assert_major_status
+    (verify module fun_context)
+    (fun status =>
+      match status with
+      | StatusCode.TYPE_MISMATCH => true
+      | _ => false
+      end
+    ).
+
+Goal test_vec_len_wrong_type = return! tt.
+Proof. reflexivity. Qed.
+
+(*
+#[test]
+#[should_panic]
+fn test_vec_len_no_arg() {
+    let code = vec![Bytecode::VecLen(SignatureIndex(3))];
+    let mut module =
+        make_module_with_local(code, SignatureToken::Vector(Box::new(SignatureToken::U32)));
+    module.signatures.push(Signature(vec![SignatureToken::U32]));
+    let fun_context = get_fun_context(&module);
+    let _result = type_safety::verify(&module, &fun_context, &mut DummyMeter);
+}
+*)
+Definition test_vec_len_no_arg : M!? _ unit :=
+  let code := [Bytecode.VecLen (SignatureIndex.Build_t 3)] in
+  let module := make_module_with_local code (SignatureToken.Vector SignatureToken.U32) in
+  let module := module <|
+    CompiledModule.signatures :=
+      module.(CompiledModule.signatures) ++ [Signature.Build_t [SignatureToken.U32]]
+  |> in
+  let! fun_context := get_fun_context module in
+  verify module fun_context.
+
+Goal
+  exists (Error : Set) (error : Error),
+  test_vec_len_no_arg = panic! error.
+Proof. repeat eexists. Qed.
+
+(*
+#[test]
+fn test_vec_imm_borrow_correct_type() {
+    let code = vec![
+        Bytecode::ImmBorrowLoc(0),
+        Bytecode::LdU64(2),
+        Bytecode::VecImmBorrow(SignatureIndex(3)),
+    ];
+    let mut module =
+        make_module_with_local(code, SignatureToken::Vector(Box::new(SignatureToken::U32)));
+    module.signatures.push(Signature(vec![SignatureToken::U32]));
+    let fun_context = get_fun_context(&module);
+    let result = type_safety::verify(&module, &fun_context, &mut DummyMeter);
+    assert!(result.is_ok());
+
+    let code = vec![
+        Bytecode::MutBorrowLoc(0),
+        Bytecode::LdU64(2),
+        Bytecode::VecImmBorrow(SignatureIndex(3)),
+    ];
+    let mut module =
+        make_module_with_local(code, SignatureToken::Vector(Box::new(SignatureToken::U32)));
+    module.signatures.push(Signature(vec![SignatureToken::U32]));
+    let fun_context = get_fun_context(&module);
+    let result = type_safety::verify(&module, &fun_context, &mut DummyMeter);
+    assert!(result.is_ok());
+}
+*)
+Definition test_vec_imm_borrow_correct_type : M! unit :=
+  let code := [
+    Bytecode.ImmBorrowLoc 0;
+    Bytecode.LdU64 2;
+    Bytecode.VecImmBorrow (SignatureIndex.Build_t 3)
+  ] in
+  let module := make_module_with_local code (SignatureToken.Vector SignatureToken.U32) in
+  let module := module <|
+    CompiledModule.signatures :=
+      module.(CompiledModule.signatures) ++ [Signature.Build_t [SignatureToken.U32]]
+  |> in
+  let! fun_context := get_fun_context module in
+  let! result := verify module fun_context in
+  do! assert_is_ok result in
+  let code := [
+    Bytecode.MutBorrowLoc 0;
+    Bytecode.LdU64 2;
+    Bytecode.VecImmBorrow (SignatureIndex.Build_t 3)
+  ] in
+  let module := make_module_with_local code (SignatureToken.Vector SignatureToken.U32) in
+  let module := module <|
+    CompiledModule.signatures :=
+      module.(CompiledModule.signatures) ++ [Signature.Build_t [SignatureToken.U32]]
+  |> in
+  let! fun_context := get_fun_context module in
+  let! result := verify module fun_context in
+  assert_is_ok result.
+
+Goal test_vec_imm_borrow_correct_type = return! tt.
+Proof. reflexivity. Qed.
+
+(*
+#[test]
+fn test_vec_imm_borrow_type_mismatch() {
+    let code = vec![
+        Bytecode::ImmBorrowLoc(0),
+        Bytecode::LdU64(2),
+        Bytecode::VecImmBorrow(SignatureIndex(3)),
+    ];
+    let mut module =
+        make_module_with_local(code, SignatureToken::Vector(Box::new(SignatureToken::U32)));
+    module.signatures.push(Signature(vec![SignatureToken::U64]));
+    let fun_context = get_fun_context(&module);
+    let result = type_safety::verify(&module, &fun_context, &mut DummyMeter);
+    assert_eq!(
+        result.unwrap_err().major_status(),
+        StatusCode::TYPE_MISMATCH
+    );
+}
+*)
+Definition test_vec_imm_borrow_type_mismatch : M! unit :=
+  let code := [
+    Bytecode.ImmBorrowLoc 0;
+    Bytecode.LdU64 2;
+    Bytecode.VecImmBorrow (SignatureIndex.Build_t 3)
+  ] in
+  let module := make_module_with_local code (SignatureToken.Vector SignatureToken.U32) in
+  let module := module <|
+    CompiledModule.signatures :=
+      module.(CompiledModule.signatures) ++ [Signature.Build_t [SignatureToken.U64]]
+  |> in
+  let! fun_context := get_fun_context module in
+  assert_major_status
+    (verify module fun_context)
+    (fun status =>
+      match status with
+      | StatusCode.TYPE_MISMATCH => true
+      | _ => false
+      end
+    ).
+
+Goal test_vec_imm_borrow_type_mismatch = return! tt.
+Proof. reflexivity. Qed.
+
+(*
+#[test]
+fn test_vec_imm_borrow_wrong_type() {
+    let code = vec![
+        Bytecode::LdU32(42),
+        Bytecode::LdU64(2),
+        Bytecode::VecImmBorrow(SignatureIndex(3)),
+    ];
+    let mut module =
+        make_module_with_local(code, SignatureToken::Vector(Box::new(SignatureToken::U32)));
+    module.signatures.push(Signature(vec![SignatureToken::U32]));
+    let fun_context = get_fun_context(&module);
+    let result = type_safety::verify(&module, &fun_context, &mut DummyMeter);
+    assert_eq!(
+        result.unwrap_err().major_status(),
+        StatusCode::TYPE_MISMATCH
+    );
+
+    let code = vec![
+        Bytecode::ImmBorrowLoc(0),
+        Bytecode::LdU32(2),
+        Bytecode::VecImmBorrow(SignatureIndex(3)),
+    ];
+    let mut module =
+        make_module_with_local(code, SignatureToken::Vector(Box::new(SignatureToken::U32)));
+    module.signatures.push(Signature(vec![SignatureToken::U32]));
+    let fun_context = get_fun_context(&module);
+    let result = type_safety::verify(&module, &fun_context, &mut DummyMeter);
+    assert_eq!(
+        result.unwrap_err().major_status(),
+        StatusCode::TYPE_MISMATCH
+    );
+}
+*)
+Definition test_vec_imm_borrow_wrong_type : M! unit :=
+  let code := [
+    Bytecode.LdU32 42;
+    Bytecode.LdU64 2;
+    Bytecode.VecImmBorrow (SignatureIndex.Build_t 3)
+  ] in
+  let module := make_module_with_local code (SignatureToken.Vector SignatureToken.U32) in
+  let module := module <|
+    CompiledModule.signatures :=
+      module.(CompiledModule.signatures) ++ [Signature.Build_t [SignatureToken.U32]]
+  |> in
+  let! fun_context := get_fun_context module in
+  do! assert_major_status
+    (verify module fun_context)
+    (fun status =>
+      match status with
+      | StatusCode.TYPE_MISMATCH => true
+      | _ => false
+      end
+    ) in
+  let code := [
+    Bytecode.ImmBorrowLoc 0;
+    Bytecode.LdU32 2;
+    Bytecode.VecImmBorrow (SignatureIndex.Build_t 3)
+  ] in
+  let module := make_module_with_local code (SignatureToken.Vector SignatureToken.U32) in
+  let module := module <|
+    CompiledModule.signatures :=
+      module.(CompiledModule.signatures) ++ [Signature.Build_t [SignatureToken.U32]]
+  |> in
+  let! fun_context := get_fun_context module in
+  assert_major_status
+    (verify module fun_context)
+    (fun status =>
+      match status with
+      | StatusCode.TYPE_MISMATCH => true
+      | _ => false
+      end
+    ).
+
+Goal test_vec_imm_borrow_wrong_type = return! tt.
+Proof. reflexivity. Qed.
+
+(*
+#[test]
+#[should_panic]
+fn test_vec_imm_borrow_too_few_args() {
+    let code = vec![
+        Bytecode::ImmBorrowLoc(0),
+        Bytecode::VecImmBorrow(SignatureIndex(3)),
+    ];
+    let mut module =
+        make_module_with_local(code, SignatureToken::Vector(Box::new(SignatureToken::U32)));
+    module.signatures.push(Signature(vec![SignatureToken::U32]));
+    let fun_context = get_fun_context(&module);
+    let _result = type_safety::verify(&module, &fun_context, &mut DummyMeter);
+}
+*)
+Definition test_vec_imm_borrow_too_few_args : M!? _ unit :=
+  let code := [
+    Bytecode.ImmBorrowLoc 0;
+    Bytecode.VecImmBorrow (SignatureIndex.Build_t 3)
+  ] in
+  let module := make_module_with_local code (SignatureToken.Vector SignatureToken.U32) in
+  let module := module <|
+    CompiledModule.signatures :=
+      module.(CompiledModule.signatures) ++ [Signature.Build_t [SignatureToken.U32]]
+  |> in
+  let! fun_context := get_fun_context module in
+  verify module fun_context.
+
+Goal
+  exists (Error : Set) (error : Error),
+  test_vec_imm_borrow_too_few_args = panic! error.
+Proof. repeat eexists. Qed.
+
+(*
+#[test]
+#[should_panic]
+fn test_vec_imm_borrow_no_arg() {
+    let code = vec![Bytecode::VecImmBorrow(SignatureIndex(3))];
+    let mut module =
+        make_module_with_local(code, SignatureToken::Vector(Box::new(SignatureToken::U32)));
+    module.signatures.push(Signature(vec![SignatureToken::U32]));
+    let fun_context = get_fun_context(&module);
+    let _result = type_safety::verify(&module, &fun_context, &mut DummyMeter);
+}
+*)
+Definition test_vec_imm_borrow_no_arg : M!? _ unit :=
+  let code := [Bytecode.VecImmBorrow (SignatureIndex.Build_t 3)] in
+  let module := make_module_with_local code (SignatureToken.Vector SignatureToken.U32) in
+  let module := module <|
+    CompiledModule.signatures :=
+      module.(CompiledModule.signatures) ++ [Signature.Build_t [SignatureToken.U32]]
+  |> in
+  let! fun_context := get_fun_context module in
+  verify module fun_context.
+
+Goal
+  exists (Error : Set) (error : Error),
+  test_vec_imm_borrow_no_arg = panic! error.
+Proof. repeat eexists. Qed.
+
+(*
+#[test]
+fn test_vec_mut_borrow_correct_type() {
+    let code = vec![
+        Bytecode::MutBorrowLoc(0),
+        Bytecode::LdU64(2),
+        Bytecode::VecMutBorrow(SignatureIndex(3)),
+    ];
+    let mut module =
+        make_module_with_local(code, SignatureToken::Vector(Box::new(SignatureToken::U32)));
+    module.signatures.push(Signature(vec![SignatureToken::U32]));
+    let fun_context = get_fun_context(&module);
+    let result = type_safety::verify(&module, &fun_context, &mut DummyMeter);
+    assert!(result.is_ok());
+}
+*)
+Definition test_vec_mut_borrow_correct_type : M! unit :=
+  let code := [
+    Bytecode.MutBorrowLoc 0;
+    Bytecode.LdU64 2;
+    Bytecode.VecMutBorrow (SignatureIndex.Build_t 3)
+  ] in
+  let module := make_module_with_local code (SignatureToken.Vector SignatureToken.U32) in
+  let module := module <|
+    CompiledModule.signatures :=
+      module.(CompiledModule.signatures) ++ [Signature.Build_t [SignatureToken.U32]]
+  |> in
+  let! fun_context := get_fun_context module in
+  let! result := verify module fun_context in
+  assert_is_ok result.
+
+Goal test_vec_mut_borrow_correct_type = return! tt.
+Proof. reflexivity. Qed.
+
+(*
+#[test]
+fn test_vec_mut_borrow_type_mismatch() {
+    let code = vec![
+        Bytecode::MutBorrowLoc(0),
+        Bytecode::LdU64(2),
+        Bytecode::VecMutBorrow(SignatureIndex(3)),
+    ];
+    let mut module =
+        make_module_with_local(code, SignatureToken::Vector(Box::new(SignatureToken::U32)));
+    module.signatures.push(Signature(vec![SignatureToken::U64]));
+    let fun_context = get_fun_context(&module);
+    let result = type_safety::verify(&module, &fun_context, &mut DummyMeter);
+    assert_eq!(
+        result.unwrap_err().major_status(),
+        StatusCode::TYPE_MISMATCH
+    );
+}
+*)
+Definition test_vec_mut_borrow_type_mismatch : M! unit :=
+  let code := [
+    Bytecode.MutBorrowLoc 0;
+    Bytecode.LdU64 2;
+    Bytecode.VecMutBorrow (SignatureIndex.Build_t 3)
+  ] in
+  let module := make_module_with_local code (SignatureToken.Vector SignatureToken.U32) in
+  let module := module <|
+    CompiledModule.signatures :=
+      module.(CompiledModule.signatures) ++ [Signature.Build_t [SignatureToken.U64]]
+  |> in
+  let! fun_context := get_fun_context module in
+  assert_major_status
+    (verify module fun_context)
+    (fun status =>
+      match status with
+      | StatusCode.TYPE_MISMATCH => true
+      | _ => false
+      end
+    ).
+
+Goal test_vec_mut_borrow_type_mismatch = return! tt.
+Proof. reflexivity. Qed.
+
+(*
+#[test]
+fn test_vec_mut_borrow_wrong_type() {
+    let code = vec![
+        Bytecode::LdU32(42),
+        Bytecode::LdU64(2),
+        Bytecode::VecMutBorrow(SignatureIndex(3)),
+    ];
+    let mut module =
+        make_module_with_local(code, SignatureToken::Vector(Box::new(SignatureToken::U32)));
+    module.signatures.push(Signature(vec![SignatureToken::U32]));
+    let fun_context = get_fun_context(&module);
+    let result = type_safety::verify(&module, &fun_context, &mut DummyMeter);
+    assert_eq!(
+        result.unwrap_err().major_status(),
+        StatusCode::TYPE_MISMATCH
+    );
+
+    let code = vec![
+        Bytecode::ImmBorrowLoc(0),
+        Bytecode::LdU64(2),
+        Bytecode::VecMutBorrow(SignatureIndex(3)),
+    ];
+    let mut module =
+        make_module_with_local(code, SignatureToken::Vector(Box::new(SignatureToken::U32)));
+    module.signatures.push(Signature(vec![SignatureToken::U32]));
+    let fun_context = get_fun_context(&module);
+    let result = type_safety::verify(&module, &fun_context, &mut DummyMeter);
+    assert_eq!(
+        result.unwrap_err().major_status(),
+        StatusCode::TYPE_MISMATCH
+    );
+
+    let code = vec![
+        Bytecode::MutBorrowLoc(0),
+        Bytecode::LdU32(2),
+        Bytecode::VecMutBorrow(SignatureIndex(3)),
+    ];
+    let mut module =
+        make_module_with_local(code, SignatureToken::Vector(Box::new(SignatureToken::U32)));
+    module.signatures.push(Signature(vec![SignatureToken::U32]));
+    let fun_context = get_fun_context(&module);
+    let result = type_safety::verify(&module, &fun_context, &mut DummyMeter);
+    assert_eq!(
+        result.unwrap_err().major_status(),
+        StatusCode::TYPE_MISMATCH
+    );
+}
+*)
+Definition test_vec_mut_borrow_wrong_type : M! unit :=
+  let code := [
+    Bytecode.LdU32 42;
+    Bytecode.LdU64 2;
+    Bytecode.VecMutBorrow (SignatureIndex.Build_t 3)
+  ] in
+  let module := make_module_with_local code (SignatureToken.Vector SignatureToken.U32) in
+  let module := module <|
+    CompiledModule.signatures :=
+      module.(CompiledModule.signatures) ++ [Signature.Build_t [SignatureToken.U32]]
+  |> in
+  let! fun_context := get_fun_context module in
+  do! assert_major_status
+    (verify module fun_context)
+    (fun status =>
+      match status with
+      | StatusCode.TYPE_MISMATCH => true
+      | _ => false
+      end
+    ) in
+  let code := [
+    Bytecode.ImmBorrowLoc 0;
+    Bytecode.LdU64 2;
+    Bytecode.VecMutBorrow (SignatureIndex.Build_t 3)
+  ] in
+  let module := make_module_with_local code (SignatureToken.Vector SignatureToken.U32) in
+  let module := module <|
+    CompiledModule.signatures :=
+      module.(CompiledModule.signatures) ++ [Signature.Build_t [SignatureToken.U32]]
+  |> in
+  let! fun_context := get_fun_context module in
+  do! assert_major_status
+    (verify module fun_context)
+    (fun status =>
+      match status with
+      | StatusCode.TYPE_MISMATCH => true
+      | _ => false
+      end
+    ) in
+  let code := [
+    Bytecode.MutBorrowLoc 0;
+    Bytecode.LdU32 2;
+    Bytecode.VecMutBorrow (SignatureIndex.Build_t 3)
+  ] in
+  let module := make_module_with_local code (SignatureToken.Vector SignatureToken.U32) in
+  let module := module <|
+    CompiledModule.signatures :=
+      module.(CompiledModule.signatures) ++ [Signature.Build_t [SignatureToken.U32]]
+  |> in
+  let! fun_context := get_fun_context module in
+  assert_major_status
+    (verify module fun_context)
+    (fun status =>
+      match status with
+      | StatusCode.TYPE_MISMATCH => true
+      | _ => false
+      end
+    ).
+
+Goal test_vec_mut_borrow_wrong_type = return! tt.
+Proof. reflexivity. Qed.
+
+(*
+#[test]
+#[should_panic]
+fn test_vec_mut_borrow_too_few_args() {
+    let code = vec![
+        Bytecode::MutBorrowLoc(0),
+        Bytecode::VecMutBorrow(SignatureIndex(3)),
+    ];
+    let mut module =
+        make_module_with_local(code, SignatureToken::Vector(Box::new(SignatureToken::U32)));
+    module.signatures.push(Signature(vec![SignatureToken::U32]));
+    let fun_context = get_fun_context(&module);
+    let _result = type_safety::verify(&module, &fun_context, &mut DummyMeter);
+}
+*)
+Definition test_vec_mut_borrow_too_few_args : M!? _ unit :=
+  let code := [
+    Bytecode.MutBorrowLoc 0;
+    Bytecode.VecMutBorrow (SignatureIndex.Build_t 3)
+  ] in
+  let module := make_module_with_local code (SignatureToken.Vector SignatureToken.U32) in
+  let module := module <|
+    CompiledModule.signatures :=
+      module.(CompiledModule.signatures) ++ [Signature.Build_t [SignatureToken.U32]]
+  |> in
+  let! fun_context := get_fun_context module in
+  verify module fun_context.
+
+Goal
+  exists (Error : Set) (error : Error),
+  test_vec_mut_borrow_too_few_args = panic! error.
+Proof. repeat eexists. Qed.
+
+(*
+#[test]
+#[should_panic]
+fn test_vec_mut_borrow_no_arg() {
+    let code = vec![Bytecode::VecMutBorrow(SignatureIndex(3))];
+    let mut module =
+        make_module_with_local(code, SignatureToken::Vector(Box::new(SignatureToken::U32)));
+    module.signatures.push(Signature(vec![SignatureToken::U32]));
+    let fun_context = get_fun_context(&module);
+    let _result = type_safety::verify(&module, &fun_context, &mut DummyMeter);
+}
+*)
+Definition test_vec_mut_borrow_no_arg : M!? _ unit :=
+  let code := [Bytecode.VecMutBorrow (SignatureIndex.Build_t 3)] in
+  let module := make_module_with_local code (SignatureToken.Vector SignatureToken.U32) in
+  let module := module <|
+    CompiledModule.signatures :=
+      module.(CompiledModule.signatures) ++ [Signature.Build_t [SignatureToken.U32]]
+  |> in
+  let! fun_context := get_fun_context module in
+  verify module fun_context.
+
+Goal
+  exists (Error : Set) (error : Error),
+  test_vec_mut_borrow_no_arg = panic! error.
+Proof. repeat eexists. Qed.
+
+(*
+#[test]
+fn test_vec_push_back_correct_type() {
+    let code = vec![
+        Bytecode::MutBorrowLoc(0),
+        Bytecode::LdU32(42),
+        Bytecode::VecPushBack(SignatureIndex(3)),
+    ];
+    let mut module =
+        make_module_with_local(code, SignatureToken::Vector(Box::new(SignatureToken::U32)));
+    module.signatures.push(Signature(vec![SignatureToken::U32]));
+    let fun_context = get_fun_context(&module);
+    let result = type_safety::verify(&module, &fun_context, &mut DummyMeter);
+    assert!(result.is_ok());
+}
+*)
+Definition test_vec_push_back_correct_type : M! unit :=
+  let code := [
+    Bytecode.MutBorrowLoc 0;
+    Bytecode.LdU32 42;
+    Bytecode.VecPushBack (SignatureIndex.Build_t 3)
+  ] in
+  let module := make_module_with_local code (SignatureToken.Vector SignatureToken.U32) in
+  let module := module <|
+    CompiledModule.signatures :=
+      module.(CompiledModule.signatures) ++ [Signature.Build_t [SignatureToken.U32]]
+  |> in
+  let! fun_context := get_fun_context module in
+  let! result := verify module fun_context in
+  assert_is_ok result.
+
+Goal test_vec_push_back_correct_type = return! tt.
+Proof. reflexivity. Qed.
+
+(*
+#[test]
+fn test_vec_push_back_type_mismatch() {
+    let code = vec![
+        Bytecode::MutBorrowLoc(0),
+        Bytecode::LdFalse,
+        Bytecode::VecPushBack(SignatureIndex(3)),
+    ];
+    let mut module =
+        make_module_with_local(code, SignatureToken::Vector(Box::new(SignatureToken::U32)));
+    module.signatures.push(Signature(vec![SignatureToken::U32]));
+    let fun_context = get_fun_context(&module);
+    let result = type_safety::verify(&module, &fun_context, &mut DummyMeter);
+    assert_eq!(
+        result.unwrap_err().major_status(),
+        StatusCode::TYPE_MISMATCH
+    );
+
+    let code = vec![
+        Bytecode::MutBorrowLoc(0),
+        Bytecode::LdU32(51),
+        Bytecode::VecPushBack(SignatureIndex(3)),
+    ];
+    let mut module =
+        make_module_with_local(code, SignatureToken::Vector(Box::new(SignatureToken::U64)));
+    module.signatures.push(Signature(vec![SignatureToken::U32]));
+    let fun_context = get_fun_context(&module);
+    let result = type_safety::verify(&module, &fun_context, &mut DummyMeter);
+    assert_eq!(
+        result.unwrap_err().major_status(),
+        StatusCode::TYPE_MISMATCH
+    );
+
+    let code = vec![
+        Bytecode::MutBorrowLoc(0),
+        Bytecode::LdU32(51),
+        Bytecode::VecPushBack(SignatureIndex(3)),
+    ];
+    let mut module =
+        make_module_with_local(code, SignatureToken::Vector(Box::new(SignatureToken::U32)));
+    module.signatures.push(Signature(vec![SignatureToken::U64]));
+    let fun_context = get_fun_context(&module);
+    let result = type_safety::verify(&module, &fun_context, &mut DummyMeter);
+    assert_eq!(
+        result.unwrap_err().major_status(),
+        StatusCode::TYPE_MISMATCH
+    );
+}
+*)
+Definition test_vec_push_back_type_mismatch : M! unit :=
+  let code := [
+    Bytecode.MutBorrowLoc 0;
+    Bytecode.LdFalse;
+    Bytecode.VecPushBack (SignatureIndex.Build_t 3)
+  ] in
+  let module := make_module_with_local code (SignatureToken.Vector SignatureToken.U32) in
+  let module := module <|
+    CompiledModule.signatures :=
+      module.(CompiledModule.signatures) ++ [Signature.Build_t [SignatureToken.U32]]
+  |> in
+  let! fun_context := get_fun_context module in
+  do! assert_major_status
+    (verify module fun_context)
+    (fun status =>
+      match status with
+      | StatusCode.TYPE_MISMATCH => true
+      | _ => false
+      end
+    ) in
+  let code := [
+    Bytecode.MutBorrowLoc 0;
+    Bytecode.LdU32 51;
+    Bytecode.VecPushBack (SignatureIndex.Build_t 3)
+  ] in
+  let module := make_module_with_local code (SignatureToken.Vector SignatureToken.U64) in
+  let module := module <|
+    CompiledModule.signatures :=
+      module.(CompiledModule.signatures) ++ [Signature.Build_t [SignatureToken.U32]]
+  |> in
+  let! fun_context := get_fun_context module in
+  do! assert_major_status
+    (verify module fun_context)
+    (fun status =>
+      match status with
+      | StatusCode.TYPE_MISMATCH => true
+      | _ => false
+      end
+    ) in
+  let code := [
+    Bytecode.MutBorrowLoc 0;
+    Bytecode.LdU32 51;
+    Bytecode.VecPushBack (SignatureIndex.Build_t 3)
+  ] in
+  let module := make_module_with_local code (SignatureToken.Vector SignatureToken.U32) in
+  let module := module <|
+    CompiledModule.signatures :=
+      module.(CompiledModule.signatures) ++ [Signature.Build_t [SignatureToken.U64]]
+  |> in
+  let! fun_context := get_fun_context module in
+  assert_major_status
+    (verify module fun_context)
+    (fun status =>
+      match status with
+      | StatusCode.TYPE_MISMATCH => true
+      | _ => false
+      end
+    ).
+
+Goal test_vec_push_back_type_mismatch = return! tt.
+Proof. reflexivity. Qed.
+
+(*
+#[test]
+fn test_vec_push_back_wrong_type() {
+    let code = vec![
+        Bytecode::LdTrue,
+        Bytecode::LdU32(42),
+        Bytecode::VecPushBack(SignatureIndex(3)),
+    ];
+    let mut module =
+        make_module_with_local(code, SignatureToken::Vector(Box::new(SignatureToken::U32)));
+    module.signatures.push(Signature(vec![SignatureToken::U32]));
+    let fun_context = get_fun_context(&module);
+    let result = type_safety::verify(&module, &fun_context, &mut DummyMeter);
+    assert_eq!(
+        result.unwrap_err().major_status(),
+        StatusCode::TYPE_MISMATCH
+    );
+
+    let code = vec![
+        Bytecode::ImmBorrowLoc(0),
+        Bytecode::LdU32(42),
+        Bytecode::VecPushBack(SignatureIndex(3)),
+    ];
+    let mut module =
+        make_module_with_local(code, SignatureToken::Vector(Box::new(SignatureToken::U32)));
+    module.signatures.push(Signature(vec![SignatureToken::U32]));
+    let fun_context = get_fun_context(&module);
+    let result = type_safety::verify(&module, &fun_context, &mut DummyMeter);
+    assert_eq!(
+        result.unwrap_err().major_status(),
+        StatusCode::TYPE_MISMATCH
+    );
+}
+*)
+Definition test_vec_push_back_wrong_type : M! unit :=
+  let code := [
+    Bytecode.LdTrue;
+    Bytecode.LdU32 42;
+    Bytecode.VecPushBack (SignatureIndex.Build_t 3)
+  ] in
+  let module := make_module_with_local code (SignatureToken.Vector SignatureToken.U32) in
+  let module := module <|
+    CompiledModule.signatures :=
+      module.(CompiledModule.signatures) ++ [Signature.Build_t [SignatureToken.U32]]
+  |> in
+  let! fun_context := get_fun_context module in
+  do! assert_major_status
+    (verify module fun_context)
+    (fun status =>
+      match status with
+      | StatusCode.TYPE_MISMATCH => true
+      | _ => false
+      end
+    ) in
+  let code := [
+    Bytecode.ImmBorrowLoc 0;
+    Bytecode.LdU32 42;
+    Bytecode.VecPushBack (SignatureIndex.Build_t 3)
+  ] in
+  let module := make_module_with_local code (SignatureToken.Vector SignatureToken.U32) in
+  let module := module <|
+    CompiledModule.signatures :=
+      module.(CompiledModule.signatures) ++ [Signature.Build_t [SignatureToken.U32]]
+  |> in
+  let! fun_context := get_fun_context module in
+  assert_major_status
+    (verify module fun_context)
+    (fun status =>
+      match status with
+      | StatusCode.TYPE_MISMATCH => true
+      | _ => false
+      end
+    ).
+
+Goal test_vec_push_back_wrong_type = return! tt.
+Proof. reflexivity. Qed.
+
+(*
+#[test]
+#[should_panic]
+fn test_vec_push_back_too_few_args() {
+    let code = vec![
+        Bytecode::MutBorrowLoc(0),
+        Bytecode::VecPushBack(SignatureIndex(3)),
+    ];
+    let mut module =
+        make_module_with_local(code, SignatureToken::Vector(Box::new(SignatureToken::U32)));
+    module.signatures.push(Signature(vec![SignatureToken::U32]));
+    let fun_context = get_fun_context(&module);
+    let _result = type_safety::verify(&module, &fun_context, &mut DummyMeter);
+}
+*)
+Definition test_vec_push_back_too_few_args : M!? _ unit :=
+  let code := [
+    Bytecode.MutBorrowLoc 0;
+    Bytecode.VecPushBack (SignatureIndex.Build_t 3)
+  ] in
+  let module := make_module_with_local code (SignatureToken.Vector SignatureToken.U32) in
+  let module := module <|
+    CompiledModule.signatures :=
+      module.(CompiledModule.signatures) ++ [Signature.Build_t [SignatureToken.U32]]
+  |> in
+  let! fun_context := get_fun_context module in
+  verify module fun_context.
+
+Goal
+  exists (Error : Set) (error : Error),
+  test_vec_push_back_too_few_args = panic! error.
+Proof. repeat eexists. Qed.
+
+(*
+#[test]
+#[should_panic]
+fn test_vec_push_back_no_arg() {
+    let code = vec![Bytecode::VecPushBack(SignatureIndex(3))];
+    let mut module =
+        make_module_with_local(code, SignatureToken::Vector(Box::new(SignatureToken::U32)));
+    module.signatures.push(Signature(vec![SignatureToken::U32]));
+    let fun_context = get_fun_context(&module);
+    let _result = type_safety::verify(&module, &fun_context, &mut DummyMeter);
+}
+*)
+Definition test_vec_push_back_no_arg : M!? _ unit :=
+  let code := [Bytecode.VecPushBack (SignatureIndex.Build_t 3)] in
+  let module := make_module_with_local code (SignatureToken.Vector SignatureToken.U32) in
+  let module := module <|
+    CompiledModule.signatures :=
+      module.(CompiledModule.signatures) ++ [Signature.Build_t [SignatureToken.U32]]
+  |> in
+  let! fun_context := get_fun_context module in
+  verify module fun_context.
+
+Goal
+  exists (Error : Set) (error : Error),
+  test_vec_push_back_no_arg = panic! error.
+Proof. repeat eexists. Qed.
+
+(*
+#[test]
+fn test_vec_pop_back_correct_type() {
+    let code = vec![
+        Bytecode::MutBorrowLoc(0),
+        Bytecode::VecPopBack(SignatureIndex(3)),
+    ];
+    let mut module =
+        make_module_with_local(code, SignatureToken::Vector(Box::new(SignatureToken::U32)));
+    module.signatures.push(Signature(vec![SignatureToken::U32]));
+    let fun_context = get_fun_context(&module);
+    let result = type_safety::verify(&module, &fun_context, &mut DummyMeter);
+    assert!(result.is_ok());
+}
+*)
+Definition test_vec_pop_back_correct_type : M! unit :=
+  let code := [
+    Bytecode.MutBorrowLoc 0;
+    Bytecode.VecPopBack (SignatureIndex.Build_t 3)
+  ] in
+  let module := make_module_with_local code (SignatureToken.Vector SignatureToken.U32) in
+  let module := module <|
+    CompiledModule.signatures :=
+      module.(CompiledModule.signatures) ++ [Signature.Build_t [SignatureToken.U32]]
+  |> in
+  let! fun_context := get_fun_context module in
+  let! result := verify module fun_context in
+  assert_is_ok result.
+
+Goal test_vec_pop_back_correct_type = return! tt.
+Proof. reflexivity. Qed.
+
+(*
+#[test]
+fn test_vec_pop_back_type_mismatch() {
+    let code = vec![
+        Bytecode::MutBorrowLoc(0),
+        Bytecode::VecPopBack(SignatureIndex(3)),
+    ];
+    let mut module =
+        make_module_with_local(code, SignatureToken::Vector(Box::new(SignatureToken::U32)));
+    module.signatures.push(Signature(vec![SignatureToken::U64]));
+    let fun_context = get_fun_context(&module);
+    let result = type_safety::verify(&module, &fun_context, &mut DummyMeter);
+    assert_eq!(
+        result.unwrap_err().major_status(),
+        StatusCode::TYPE_MISMATCH
+    );
+}
+*)
+Definition test_vec_pop_back_type_mismatch : M! unit :=
+  let code := [
+    Bytecode.MutBorrowLoc 0;
+    Bytecode.VecPopBack (SignatureIndex.Build_t 3)
+  ] in
+  let module := make_module_with_local code (SignatureToken.Vector SignatureToken.U32) in
+  let module := module <|
+    CompiledModule.signatures :=
+      module.(CompiledModule.signatures) ++ [Signature.Build_t [SignatureToken.U64]]
+  |> in
+  let! fun_context := get_fun_context module in
+  assert_major_status
+    (verify module fun_context)
+    (fun status =>
+      match status with
+      | StatusCode.TYPE_MISMATCH => true
+      | _ => false
+      end
+    ).
+
+Goal test_vec_pop_back_type_mismatch = return! tt.
+Proof. reflexivity. Qed.
+
+(*
+#[test]
+fn test_vec_pop_back_wrong_type() {
+    let code = vec![Bytecode::LdTrue, Bytecode::VecPopBack(SignatureIndex(3))];
+    let mut module =
+        make_module_with_local(code, SignatureToken::Vector(Box::new(SignatureToken::U32)));
+    module.signatures.push(Signature(vec![SignatureToken::U32]));
+    let fun_context = get_fun_context(&module);
+    let result = type_safety::verify(&module, &fun_context, &mut DummyMeter);
+    assert_eq!(
+        result.unwrap_err().major_status(),
+        StatusCode::TYPE_MISMATCH
+    );
+
+    let code = vec![
+        Bytecode::ImmBorrowLoc(0),
+        Bytecode::VecPopBack(SignatureIndex(3)),
+    ];
+    let mut module =
+        make_module_with_local(code, SignatureToken::Vector(Box::new(SignatureToken::U32)));
+    module.signatures.push(Signature(vec![SignatureToken::U32]));
+    let fun_context = get_fun_context(&module);
+    let result = type_safety::verify(&module, &fun_context, &mut DummyMeter);
+    assert_eq!(
+        result.unwrap_err().major_status(),
+        StatusCode::TYPE_MISMATCH
+    );
+}
+*)
+Definition test_vec_pop_back_wrong_type : M! unit :=
+  let code := [Bytecode.LdTrue; Bytecode.VecPopBack (SignatureIndex.Build_t 3)] in
+  let module := make_module_with_local code (SignatureToken.Vector SignatureToken.U32) in
+  let module := module <|
+    CompiledModule.signatures :=
+      module.(CompiledModule.signatures) ++ [Signature.Build_t [SignatureToken.U32]]
+  |> in
+  let! fun_context := get_fun_context module in
+  do! assert_major_status
+    (verify module fun_context)
+    (fun status =>
+      match status with
+      | StatusCode.TYPE_MISMATCH => true
+      | _ => false
+      end
+    ) in
+  let code := [
+    Bytecode.ImmBorrowLoc 0;
+    Bytecode.VecPopBack (SignatureIndex.Build_t 3)
+  ] in
+  let module := make_module_with_local code (SignatureToken.Vector SignatureToken.U32) in
+  let module := module <|
+    CompiledModule.signatures :=
+      module.(CompiledModule.signatures) ++ [Signature.Build_t [SignatureToken.U32]]
+  |> in
+  let! fun_context := get_fun_context module in
+  assert_major_status
+    (verify module fun_context)
+    (fun status =>
+      match status with
+      | StatusCode.TYPE_MISMATCH => true
+      | _ => false
+      end
+    ).
+
+Goal test_vec_pop_back_wrong_type = return! tt.
+Proof. reflexivity. Qed.
+
+(*
+#[test]
+#[should_panic]
+fn test_vec_pop_back_no_arg() {
+    let code = vec![Bytecode::VecPopBack(SignatureIndex(3))];
+    let mut module =
+        make_module_with_local(code, SignatureToken::Vector(Box::new(SignatureToken::U32)));
+    module.signatures.push(Signature(vec![SignatureToken::U32]));
+    let fun_context = get_fun_context(&module);
+    let _result = type_safety::verify(&module, &fun_context, &mut DummyMeter);
+}
+*)
+Definition test_vec_pop_back_no_arg : M!? _ unit :=
+  let code := [Bytecode.VecPopBack (SignatureIndex.Build_t 3)] in
+  let module := make_module_with_local code (SignatureToken.Vector SignatureToken.U32) in
+  let module := module <|
+    CompiledModule.signatures :=
+      module.(CompiledModule.signatures) ++ [Signature.Build_t [SignatureToken.U32]]
+  |> in
+  let! fun_context := get_fun_context module in
+  verify module fun_context.
+
+Goal
+  exists (Error : Set) (error : Error),
+  test_vec_pop_back_no_arg = panic! error.
+Proof. repeat eexists. Qed.
+
+(*
+#[test]
+fn test_vec_swap_correct_type() {
+    let code = vec![
+        Bytecode::MutBorrowLoc(0),
+        Bytecode::LdU64(2),
+        Bytecode::LdU64(3),
+        Bytecode::VecSwap(SignatureIndex(3)),
+    ];
+    let mut module =
+        make_module_with_local(code, SignatureToken::Vector(Box::new(SignatureToken::U32)));
+    module.signatures.push(Signature(vec![SignatureToken::U32]));
+    let fun_context = get_fun_context(&module);
+    let result = type_safety::verify(&module, &fun_context, &mut DummyMeter);
+    assert!(result.is_ok());
+}
+*)
+Definition test_vec_swap_correct_type : M! unit :=
+  let code := [
+    Bytecode.MutBorrowLoc 0;
+    Bytecode.LdU64 2;
+    Bytecode.LdU64 3;
+    Bytecode.VecSwap (SignatureIndex.Build_t 3)
+  ] in
+  let module := make_module_with_local code (SignatureToken.Vector SignatureToken.U32) in
+  let module := module <|
+    CompiledModule.signatures :=
+      module.(CompiledModule.signatures) ++ [Signature.Build_t [SignatureToken.U32]]
+  |> in
+  let! fun_context := get_fun_context module in
+  let! result := verify module fun_context in
+  assert_is_ok result.
+
+Goal test_vec_swap_correct_type = return! tt.
+Proof. reflexivity. Qed.
+
+(*
+#[test]
+fn test_vec_swap_type_mismatch() {
+    let code = vec![
+        Bytecode::MutBorrowLoc(0),
+        Bytecode::LdU64(2),
+        Bytecode::LdU64(3),
+        Bytecode::VecSwap(SignatureIndex(3)),
+    ];
+    let mut module =
+        make_module_with_local(code, SignatureToken::Vector(Box::new(SignatureToken::U32)));
+    module.signatures.push(Signature(vec![SignatureToken::U64]));
+    let fun_context = get_fun_context(&module);
+    let result = type_safety::verify(&module, &fun_context, &mut DummyMeter);
+    assert_eq!(
+        result.unwrap_err().major_status(),
+        StatusCode::TYPE_MISMATCH
+    );
+}
+*)
+Definition test_vec_swap_type_mismatch : M! unit :=
+  let code := [
+    Bytecode.MutBorrowLoc 0;
+    Bytecode.LdU64 2;
+    Bytecode.LdU64 3;
+    Bytecode.VecSwap (SignatureIndex.Build_t 3)
+  ] in
+  let module := make_module_with_local code (SignatureToken.Vector SignatureToken.U32) in
+  let module := module <|
+    CompiledModule.signatures :=
+      module.(CompiledModule.signatures) ++ [Signature.Build_t [SignatureToken.U64]]
+  |> in
+  let! fun_context := get_fun_context module in
+  assert_major_status
+    (verify module fun_context)
+    (fun status =>
+      match status with
+      | StatusCode.TYPE_MISMATCH => true
+      | _ => false
+      end
+    ).
+
+Goal test_vec_swap_type_mismatch = return! tt.
+Proof. reflexivity. Qed.
+
+(*
+#[test]
+fn test_vec_swap_wrong_type() {
+*)
+Definition test_vec_swap_wrong_type : M! unit :=
+  (*
+    let code = vec![
+        Bytecode::LdTrue,
+        Bytecode::LdU64(2),
+        Bytecode::LdU64(3),
+        Bytecode::VecSwap(SignatureIndex(3)),
+    ];
+    let mut module =
+        make_module_with_local(code, SignatureToken::Vector(Box::new(SignatureToken::U32)));
+    module.signatures.push(Signature(vec![SignatureToken::U32]));
+    let fun_context = get_fun_context(&module);
+    let result = type_safety::verify(&module, &fun_context, &mut DummyMeter);
+    assert_eq!(
+        result.unwrap_err().major_status(),
+        StatusCode::TYPE_MISMATCH
+    );
+  *)
+  let code := [
+    Bytecode.LdTrue;
+    Bytecode.LdU64 2;
+    Bytecode.LdU64 3;
+    Bytecode.VecSwap (SignatureIndex.Build_t 3)
+  ] in
+  let module := make_module_with_local code (SignatureToken.Vector SignatureToken.U32) in
+  let module := module <|
+    CompiledModule.signatures :=
+      module.(CompiledModule.signatures) ++ [Signature.Build_t [SignatureToken.U32]]
+  |> in
+  let! fun_context := get_fun_context module in
+  do! assert_major_status
+    (verify module fun_context)
+    (fun status =>
+      match status with
+      | StatusCode.TYPE_MISMATCH => true
+      | _ => false
+      end
+    ) in
+  (*
+    let code = vec![
+        Bytecode::ImmBorrowLoc(0),
+        Bytecode::LdU64(2),
+        Bytecode::LdU64(3),
+        Bytecode::VecSwap(SignatureIndex(3)),
+    ];
+    let mut module =
+        make_module_with_local(code, SignatureToken::Vector(Box::new(SignatureToken::U32)));
+    module.signatures.push(Signature(vec![SignatureToken::U32]));
+    let fun_context = get_fun_context(&module);
+    let result = type_safety::verify(&module, &fun_context, &mut DummyMeter);
+    assert_eq!(
+        result.unwrap_err().major_status(),
+        StatusCode::TYPE_MISMATCH
+    );
+  *)
+  let code := [
+    Bytecode.ImmBorrowLoc 0;
+    Bytecode.LdU64 2;
+    Bytecode.LdU64 3;
+    Bytecode.VecSwap (SignatureIndex.Build_t 3)
+  ] in
+  let module := make_module_with_local code (SignatureToken.Vector SignatureToken.U32) in
+  let module := module <|
+    CompiledModule.signatures :=
+      module.(CompiledModule.signatures) ++ [Signature.Build_t [SignatureToken.U32]]
+  |> in
+  let! fun_context := get_fun_context module in
+  do! assert_major_status
+    (verify module fun_context)
+    (fun status =>
+      match status with
+      | StatusCode.TYPE_MISMATCH => true
+      | _ => false
+      end
+    ) in
+  (*
+    let code = vec![
+        Bytecode::MutBorrowLoc(0),
+        Bytecode::LdU32(2),
+        Bytecode::LdU64(3),
+        Bytecode::VecSwap(SignatureIndex(3)),
+    ];
+    let mut module =
+        make_module_with_local(code, SignatureToken::Vector(Box::new(SignatureToken::U32)));
+    module.signatures.push(Signature(vec![SignatureToken::U32]));
+    let fun_context = get_fun_context(&module);
+    let result = type_safety::verify(&module, &fun_context, &mut DummyMeter);
+    assert_eq!(
+        result.unwrap_err().major_status(),
+        StatusCode::TYPE_MISMATCH
+    );
+  *)
+  let code := [
+    Bytecode.MutBorrowLoc 0;
+    Bytecode.LdU32 2;
+    Bytecode.LdU64 3;
+    Bytecode.VecSwap (SignatureIndex.Build_t 3)
+  ] in
+  let module := make_module_with_local code (SignatureToken.Vector SignatureToken.U32) in
+  let module := module <|
+    CompiledModule.signatures :=
+      module.(CompiledModule.signatures) ++ [Signature.Build_t [SignatureToken.U32]]
+  |> in
+  let! fun_context := get_fun_context module in
+  do! assert_major_status
+    (verify module fun_context)
+    (fun status =>
+      match status with
+      | StatusCode.TYPE_MISMATCH => true
+      | _ => false
+      end
+    ) in
+  (*
+    let code = vec![
+        Bytecode::MutBorrowLoc(0),
+        Bytecode::LdU64(2),
+        Bytecode::LdU32(3),
+        Bytecode::VecSwap(SignatureIndex(3)),
+    ];
+    let mut module =
+        make_module_with_local(code, SignatureToken::Vector(Box::new(SignatureToken::U32)));
+    module.signatures.push(Signature(vec![SignatureToken::U32]));
+    let fun_context = get_fun_context(&module);
+    let result = type_safety::verify(&module, &fun_context, &mut DummyMeter);
+    assert_eq!(
+        result.unwrap_err().major_status(),
+        StatusCode::TYPE_MISMATCH
+    );
+  *)
+  let code := [
+    Bytecode.MutBorrowLoc 0;
+    Bytecode.LdU64 2;
+    Bytecode.LdU32 3;
+    Bytecode.VecSwap (SignatureIndex.Build_t 3)
+  ] in
+  let module := make_module_with_local code (SignatureToken.Vector SignatureToken.U32) in
+  let module := module <|
+    CompiledModule.signatures :=
+      module.(CompiledModule.signatures) ++ [Signature.Build_t [SignatureToken.U32]]
+  |> in
+  let! fun_context := get_fun_context module in
+  assert_major_status
+    (verify module fun_context)
+    (fun status =>
+      match status with
+      | StatusCode.TYPE_MISMATCH => true
+      | _ => false
+      end
+    ).
+
+Goal test_vec_swap_wrong_type = return! tt.
+Proof. reflexivity. Qed.
+
+(*
+#[test]
+#[should_panic]
+fn test_vec_swap_too_few_args() {
+    let code = vec![
+        Bytecode::MutBorrowLoc(0),
+        Bytecode::LdU64(2),
+        Bytecode::VecSwap(SignatureIndex(3)),
+    ];
+    let mut module =
+        make_module_with_local(code, SignatureToken::Vector(Box::new(SignatureToken::U32)));
+    module.signatures.push(Signature(vec![SignatureToken::U32]));
+    let fun_context = get_fun_context(&module);
+    let _result = type_safety::verify(&module, &fun_context, &mut DummyMeter);
+}
+*)
+Definition test_vec_swap_too_few_args : M!? _ unit :=
+  let code := [
+    Bytecode.MutBorrowLoc 0;
+    Bytecode.LdU64 2;
+    Bytecode.VecSwap (SignatureIndex.Build_t 3)
+  ] in
+  let module := make_module_with_local code (SignatureToken.Vector SignatureToken.U32) in
+  let module := module <|
+    CompiledModule.signatures :=
+      module.(CompiledModule.signatures) ++ [Signature.Build_t [SignatureToken.U32]]
+  |> in
+  let! fun_context := get_fun_context module in
+  verify module fun_context.
+
+Goal
+  exists (Error : Set) (error : Error),
+  test_vec_swap_too_few_args = panic! error.
+Proof. repeat eexists. Qed.
+
+(*
+#[test]
+#[should_panic]
+fn test_vec_swap_no_arg() {
+    let code = vec![Bytecode::VecSwap(SignatureIndex(3))];
+    let mut module =
+        make_module_with_local(code, SignatureToken::Vector(Box::new(SignatureToken::U32)));
+    module.signatures.push(Signature(vec![SignatureToken::U32]));
+    let fun_context = get_fun_context(&module);
+    let _result = type_safety::verify(&module, &fun_context, &mut DummyMeter);
+}
+*)
+Definition test_vec_swap_no_arg : M!? _ unit :=
+  let code := [Bytecode.VecSwap (SignatureIndex.Build_t 3)] in
+  let module := make_module_with_local code (SignatureToken.Vector SignatureToken.U32) in
+  let module := module <|
+    CompiledModule.signatures :=
+      module.(CompiledModule.signatures) ++ [Signature.Build_t [SignatureToken.U32]]
+  |> in
+  let! fun_context := get_fun_context module in
+  verify module fun_context.
+
+Goal
+  exists (Error : Set) (error : Error),
+  test_vec_swap_no_arg = panic! error.
+Proof. repeat eexists. Qed.
+
+(*
+#[test]
+fn test_exists_deprecated_correct_type() {
+    let code = vec![
+        Bytecode::CopyLoc(0),
+        Bytecode::ExistsDeprecated(StructDefinitionIndex(0)),
+    ];
+    let mut module = make_module_with_local(code, SignatureToken::Address);
+    add_simple_struct_with_abilities(&mut module, AbilitySet::ALL);
+    let fun_context = get_fun_context(&module);
+    let result = type_safety::verify(&module, &fun_context, &mut DummyMeter);
+    assert!(result.is_ok());
+}
+*)
+Definition test_exists_deprecated_correct_type : M! unit :=
+  let code := [
+    Bytecode.CopyLoc 0;
+    Bytecode.ExistsDeprecated (StructDefinitionIndex.Build_t 0)
+  ] in
+  let module := make_module_with_local code SignatureToken.Address in
+  let module := add_simple_struct_with_abilities module AbilitySet.ALL in
+  let! fun_context := get_fun_context module in
+  let! result := verify module fun_context in
+  assert_is_ok result.
+
+Goal test_exists_deprecated_correct_type = return! tt.
+Proof. reflexivity. Qed.
+
+(*
+#[test]
+fn test_exists_deprecated_wrong_type() {
+    let code = vec![
+        Bytecode::LdU64(42),
+        Bytecode::ExistsDeprecated(StructDefinitionIndex(0)),
+    ];
+    let mut module = make_module_with_local(code, SignatureToken::Address);
+    add_simple_struct_with_abilities(&mut module, AbilitySet::ALL);
+    let fun_context = get_fun_context(&module);
+    let result = type_safety::verify(&module, &fun_context, &mut DummyMeter);
+    assert_eq!(
+        result.unwrap_err().major_status(),
+        StatusCode::EXISTS_WITHOUT_KEY_ABILITY_OR_BAD_ARGUMENT
+    );
+}
+*)
+Definition test_exists_deprecated_wrong_type : M! unit :=
+  let code := [
+    Bytecode.LdU64 42;
+    Bytecode.ExistsDeprecated (StructDefinitionIndex.Build_t 0)
+  ] in
+  let module := make_module_with_local code SignatureToken.Address in
+  let module := add_simple_struct_with_abilities module AbilitySet.ALL in
+  let! fun_context := get_fun_context module in
+  assert_major_status
+    (verify module fun_context)
+    (fun status =>
+      match status with
+      | StatusCode.EXISTS_WITHOUT_KEY_ABILITY_OR_BAD_ARGUMENT => true
+      | _ => false
+      end
+    ).
+
+Goal test_exists_deprecated_wrong_type = return! tt.
+Proof. reflexivity. Qed.
+
+(*
+#[test]
+fn test_exists_deprecated_no_key() {
+    let code = vec![
+        Bytecode::CopyLoc(0),
+        Bytecode::ExistsDeprecated(StructDefinitionIndex(0)),
+    ];
+    let mut module = make_module_with_local(code, SignatureToken::Address);
+    add_simple_struct_with_abilities(&mut module, AbilitySet::PRIMITIVES);
+    let fun_context = get_fun_context(&module);
+    let result = type_safety::verify(&module, &fun_context, &mut DummyMeter);
+    assert_eq!(
+        result.unwrap_err().major_status(),
+        StatusCode::EXISTS_WITHOUT_KEY_ABILITY_OR_BAD_ARGUMENT
+    );
+}
+*)
+Definition test_exists_deprecated_no_key : M! unit :=
+  let code := [
+    Bytecode.CopyLoc 0;
+    Bytecode.ExistsDeprecated (StructDefinitionIndex.Build_t 0)
+  ] in
+  let module := make_module_with_local code SignatureToken.Address in
+  let module := add_simple_struct_with_abilities module AbilitySet.PRIMITIVES in
+  let! fun_context := get_fun_context module in
+  assert_major_status
+    (verify module fun_context)
+    (fun status =>
+      match status with
+      | StatusCode.EXISTS_WITHOUT_KEY_ABILITY_OR_BAD_ARGUMENT => true
+      | _ => false
+      end
+    ).
+
+Goal test_exists_deprecated_no_key = return! tt.
+Proof. reflexivity. Qed.
+
+(*
+#[test]
+#[should_panic]
+fn test_exists_deprecated_no_arg() {
+    let code = vec![Bytecode::ExistsDeprecated(StructDefinitionIndex(0))];
+    let mut module = make_module_with_local(code, SignatureToken::Address);
+    add_simple_struct_with_abilities(&mut module, AbilitySet::ALL);
+    let fun_context = get_fun_context(&module);
+    let _result = type_safety::verify(&module, &fun_context, &mut DummyMeter);
+}
+*)
+Definition test_exists_deprecated_no_arg : M!? _ unit :=
+  let code := [Bytecode.ExistsDeprecated (StructDefinitionIndex.Build_t 0)] in
+  let module := make_module_with_local code SignatureToken.Address in
+  let module := add_simple_struct_with_abilities module AbilitySet.ALL in
+  let! fun_context := get_fun_context module in
+  verify module fun_context.
+
+Goal
+  exists (Error : Set) (error : Error),
+  test_exists_deprecated_no_arg = panic! error.
+Proof. repeat eexists. Qed.
+
+(*
+#[test]
+fn test_exists_generic_deprecated_correct_type() {
+    let code = vec![
+        Bytecode::CopyLoc(0),
+        Bytecode::ExistsGenericDeprecated(StructDefInstantiationIndex(0)),
+    ];
+    let mut module = make_module_with_local(code, SignatureToken::Address);
+    add_simple_struct_generic_with_abilities(&mut module, AbilitySet::ALL, SignatureToken::U32);
+    let fun_context: FunctionContext<'_> = get_fun_context(&module);
+    let result = type_safety::verify(&module, &fun_context, &mut DummyMeter);
+    assert!(result.is_ok());
+}
+*)
+Definition test_exists_generic_deprecated_correct_type : M! unit :=
+  let code := [
+    Bytecode.CopyLoc 0;
+    Bytecode.ExistsGenericDeprecated (StructDefInstantiationIndex.Build_t 0)
+  ] in
+  let module := make_module_with_local code SignatureToken.Address in
+  let module := add_simple_struct_generic_with_abilities module AbilitySet.ALL SignatureToken.U32 in
+  let! fun_context := get_fun_context module in
+  let! result := verify module fun_context in
+  assert_is_ok result.
+
+Goal test_exists_generic_deprecated_correct_type = return! tt.
+Proof. reflexivity. Qed.
+
+(*
+#[test]
+fn test_exists_generic_deprecated_wrong_type() {
+    let code = vec![
+        Bytecode::LdU64(42),
+        Bytecode::ExistsGenericDeprecated(StructDefInstantiationIndex(0)),
+    ];
+    let mut module = make_module_with_local(code, SignatureToken::Address);
+    add_simple_struct_generic_with_abilities(&mut module, AbilitySet::ALL, SignatureToken::U32);
+    let fun_context = get_fun_context(&module);
+    let result = type_safety::verify(&module, &fun_context, &mut DummyMeter);
+    assert_eq!(
+        result.unwrap_err().major_status(),
+        StatusCode::EXISTS_WITHOUT_KEY_ABILITY_OR_BAD_ARGUMENT
+    );
+}
+*)
+Definition test_exists_generic_deprecated_wrong_type : M! unit :=
+  let code := [
+    Bytecode.LdU64 42;
+    Bytecode.ExistsGenericDeprecated (StructDefInstantiationIndex.Build_t 0)
+  ] in
+  let module := make_module_with_local code SignatureToken.Address in
+  let module := add_simple_struct_generic_with_abilities module AbilitySet.ALL SignatureToken.U32 in
+  let! fun_context := get_fun_context module in
+  assert_major_status
+    (verify module fun_context)
+    (fun status =>
+      match status with
+      | StatusCode.EXISTS_WITHOUT_KEY_ABILITY_OR_BAD_ARGUMENT => true
+      | _ => false
+      end
+    ).
+
+Goal test_exists_generic_deprecated_wrong_type = return! tt.
+Proof. reflexivity. Qed.
+
+(*
+#[test]
+fn test_exists_generic_deprecated_no_key() {
+    let code = vec![
+        Bytecode::CopyLoc(0),
+        Bytecode::ExistsGenericDeprecated(StructDefInstantiationIndex(0)),
+    ];
+    let mut module = make_module_with_local(code, SignatureToken::Address);
+    add_simple_struct_generic_with_abilities(
+        &mut module,
+        AbilitySet::PRIMITIVES,
+        SignatureToken::U32,
+    );
+    let fun_context = get_fun_context(&module);
+    let result = type_safety::verify(&module, &fun_context, &mut DummyMeter);
+    assert_eq!(
+        result.unwrap_err().major_status(),
+        StatusCode::EXISTS_WITHOUT_KEY_ABILITY_OR_BAD_ARGUMENT
+    );
+}
+*)
+Definition test_exists_generic_deprecated_no_key : M! unit :=
+  let code := [
+    Bytecode.CopyLoc 0;
+    Bytecode.ExistsGenericDeprecated (StructDefInstantiationIndex.Build_t 0)
+  ] in
+  let module := make_module_with_local code SignatureToken.Address in
+  let module := add_simple_struct_generic_with_abilities module AbilitySet.PRIMITIVES SignatureToken.U32 in
+  let! fun_context := get_fun_context module in
+  assert_major_status
+    (verify module fun_context)
+    (fun status =>
+      match status with
+      | StatusCode.EXISTS_WITHOUT_KEY_ABILITY_OR_BAD_ARGUMENT => true
+      | _ => false
+      end
+    ).
+
+Goal test_exists_generic_deprecated_no_key = return! tt.
+Proof. reflexivity. Qed.
+
+(*
+#[test]
+#[should_panic]
+fn test_exists_generic_deprecated_no_arg() {
+    let code = vec![Bytecode::ExistsGenericDeprecated(
+        StructDefInstantiationIndex(0),
+    )];
+    let mut module = make_module_with_local(code, SignatureToken::Address);
+    add_simple_struct_generic_with_abilities(&mut module, AbilitySet::ALL, SignatureToken::U32);
+    let fun_context = get_fun_context(&module);
+    let _result = type_safety::verify(&module, &fun_context, &mut DummyMeter);
+}
+*)
+Definition test_exists_generic_deprecated_no_arg : M!? _ unit :=
+  let code := [Bytecode.ExistsGenericDeprecated (StructDefInstantiationIndex.Build_t 0)] in
+  let module := make_module_with_local code SignatureToken.Address in
+  let module := add_simple_struct_generic_with_abilities module AbilitySet.ALL SignatureToken.U32 in
+  let! fun_context := get_fun_context module in
+  verify module fun_context.
+
+Goal
+  exists (Error : Set) (error : Error),
+  test_exists_generic_deprecated_no_arg = panic! error.
+Proof. repeat eexists. Qed.
+
+(*
+#[test]
+fn test_move_from_deprecated_correct_type() {
+    let code = vec![
+        Bytecode::CopyLoc(0),
+        Bytecode::MoveFromDeprecated(StructDefinitionIndex(0)),
+    ];
+    let mut module = make_module_with_local(code, SignatureToken::Address);
+    add_simple_struct_with_abilities(&mut module, AbilitySet::ALL);
+    let fun_context = get_fun_context(&module);
+    let result = type_safety::verify(&module, &fun_context, &mut DummyMeter);
+    assert!(result.is_ok());
+}
+*)
+Definition test_move_from_deprecated_correct_type : M! unit :=
+  let code := [
+    Bytecode.CopyLoc 0;
+    Bytecode.MoveFromDeprecated (StructDefinitionIndex.Build_t 0)
+  ] in
+  let module := make_module_with_local code SignatureToken.Address in
+  let module := add_simple_struct_with_abilities module AbilitySet.ALL in
+  let! fun_context := get_fun_context module in
+  let! result := verify module fun_context in
+  assert_is_ok result.
+
+Goal test_move_from_deprecated_correct_type = return! tt.
+Proof. reflexivity. Qed.
+
+(*
+#[test]
+fn test_move_from_deprecated_wrong_type() {
+    let code = vec![
+        Bytecode::LdU64(42),
+        Bytecode::MoveFromDeprecated(StructDefinitionIndex(0)),
+    ];
+    let mut module = make_module_with_local(code, SignatureToken::Address);
+    add_simple_struct_with_abilities(&mut module, AbilitySet::ALL);
+    let fun_context = get_fun_context(&module);
+    let result = type_safety::verify(&module, &fun_context, &mut DummyMeter);
+    assert_eq!(
+        result.unwrap_err().major_status(),
+        StatusCode::MOVEFROM_TYPE_MISMATCH_ERROR
+    );
+}
+*)
+Definition test_move_from_deprecated_wrong_type : M! unit :=
+  let code := [
+    Bytecode.LdU64 42;
+    Bytecode.MoveFromDeprecated (StructDefinitionIndex.Build_t 0)
+  ] in
+  let module := make_module_with_local code SignatureToken.Address in
+  let module := add_simple_struct_with_abilities module AbilitySet.ALL in
+  let! fun_context := get_fun_context module in
+  assert_major_status
+    (verify module fun_context)
+    (fun status =>
+      match status with
+      | StatusCode.MOVEFROM_TYPE_MISMATCH_ERROR => true
+      | _ => false
+      end
+    ).
+
+Goal test_move_from_deprecated_wrong_type = return! tt.
+Proof. reflexivity. Qed.
+
+(*
+#[test]
+fn test_move_from_deprecated_no_key() {
+    let code = vec![
+        Bytecode::CopyLoc(0),
+        Bytecode::MoveFromDeprecated(StructDefinitionIndex(0)),
+    ];
+    let mut module = make_module_with_local(code, SignatureToken::Address);
+    add_simple_struct_with_abilities(&mut module, AbilitySet::PRIMITIVES);
+    let fun_context = get_fun_context(&module);
+    let result = type_safety::verify(&module, &fun_context, &mut DummyMeter);
+    assert_eq!(
+        result.unwrap_err().major_status(),
+        StatusCode::MOVEFROM_WITHOUT_KEY_ABILITY
+    );
+}
+*)
+Definition test_move_from_deprecated_no_key : M! unit :=
+  let code := [
+    Bytecode.CopyLoc 0;
+    Bytecode.MoveFromDeprecated (StructDefinitionIndex.Build_t 0)
+  ] in
+  let module := make_module_with_local code SignatureToken.Address in
+  let module := add_simple_struct_with_abilities module AbilitySet.PRIMITIVES in
+  let! fun_context := get_fun_context module in
+  assert_major_status
+    (verify module fun_context)
+    (fun status =>
+      match status with
+      | StatusCode.MOVEFROM_WITHOUT_KEY_ABILITY => true
+      | _ => false
+      end
+    ).
+
+Goal test_move_from_deprecated_no_key = return! tt.
+Proof. reflexivity. Qed.
+
+(*
+#[test]
+#[should_panic]
+fn test_move_from_deprecated_no_arg() {
+    let code = vec![Bytecode::MoveFromDeprecated(StructDefinitionIndex(0))];
+    let mut module = make_module_with_local(code, SignatureToken::Address);
+    add_simple_struct_with_abilities(&mut module, AbilitySet::ALL);
+    let fun_context = get_fun_context(&module);
+    let _result = type_safety::verify(&module, &fun_context, &mut DummyMeter);
+}
+*)
+Definition test_move_from_deprecated_no_arg : M!? _ unit :=
+  let code := [Bytecode.MoveFromDeprecated (StructDefinitionIndex.Build_t 0)] in
+  let module := make_module_with_local code SignatureToken.Address in
+  let module := add_simple_struct_with_abilities module AbilitySet.ALL in
+  let! fun_context := get_fun_context module in
+  verify module fun_context.
+
+Goal
+  exists (Error : Set) (error : Error),
+  test_move_from_deprecated_no_arg = panic! error.
+Proof. repeat eexists. Qed.
+
+(*
+#[test]
+fn test_move_from_generic_deprecated_correct_type() {
+    let code = vec![
+        Bytecode::CopyLoc(0),
+        Bytecode::MoveFromGenericDeprecated(StructDefInstantiationIndex(0)),
+    ];
+    let mut module = make_module_with_local(code, SignatureToken::Address);
+    add_simple_struct_generic_with_abilities(&mut module, AbilitySet::ALL, SignatureToken::U32);
+    let fun_context = get_fun_context(&module);
+    let result = type_safety::verify(&module, &fun_context, &mut DummyMeter);
+    assert!(result.is_ok());
+}
+*)
+Definition test_move_from_generic_deprecated_correct_type : M! unit :=
+  let code := [
+    Bytecode.CopyLoc 0;
+    Bytecode.MoveFromGenericDeprecated (StructDefInstantiationIndex.Build_t 0)
+  ] in
+  let module := make_module_with_local code SignatureToken.Address in
+  let module := add_simple_struct_generic_with_abilities module AbilitySet.ALL SignatureToken.U32 in
+  let! fun_context := get_fun_context module in
+  let! result := verify module fun_context in
+  assert_is_ok result.
+
+Goal test_move_from_generic_deprecated_correct_type = return! tt.
+Proof. reflexivity. Qed.
+
+(*
+#[test]
+fn test_move_from_generic_deprecated_wrong_type() {
+    let code = vec![
+        Bytecode::LdU64(42),
+        Bytecode::MoveFromGenericDeprecated(StructDefInstantiationIndex(0)),
+    ];
+    let mut module = make_module_with_local(code, SignatureToken::Address);
+    add_simple_struct_generic_with_abilities(&mut module, AbilitySet::ALL, SignatureToken::U32);
+    let fun_context = get_fun_context(&module);
+    let result = type_safety::verify(&module, &fun_context, &mut DummyMeter);
+    assert_eq!(
+        result.unwrap_err().major_status(),
+        StatusCode::MOVEFROM_TYPE_MISMATCH_ERROR
+    );
+}
+*)
+Definition test_move_from_generic_deprecated_wrong_type : M! unit :=
+  let code := [
+    Bytecode.LdU64 42;
+    Bytecode.MoveFromGenericDeprecated (StructDefInstantiationIndex.Build_t 0)
+  ] in
+  let module := make_module_with_local code SignatureToken.Address in
+  let module := add_simple_struct_generic_with_abilities module AbilitySet.ALL SignatureToken.U32 in
+  let! fun_context := get_fun_context module in
+  assert_major_status
+    (verify module fun_context)
+    (fun status =>
+      match status with
+      | StatusCode.MOVEFROM_TYPE_MISMATCH_ERROR => true
+      | _ => false
+      end
+    ).
+
+Goal test_move_from_generic_deprecated_wrong_type = return! tt.
+Proof. reflexivity. Qed.
+
+(*
+#[test]
+fn test_move_from_generic_deprecated_no_key() {
+    let code = vec![
+        Bytecode::CopyLoc(0),
+        Bytecode::MoveFromGenericDeprecated(StructDefInstantiationIndex(0)),
+    ];
+    let mut module = make_module_with_local(code, SignatureToken::Address);
+    add_simple_struct_generic_with_abilities(
+        &mut module,
+        AbilitySet::PRIMITIVES,
+        SignatureToken::U32,
+    );
+    let fun_context = get_fun_context(&module);
+    let result = type_safety::verify(&module, &fun_context, &mut DummyMeter);
+    assert_eq!(
+        result.unwrap_err().major_status(),
+        StatusCode::MOVEFROM_WITHOUT_KEY_ABILITY
+    );
+}
+*)
+Definition test_move_from_generic_deprecated_no_key : M! unit :=
+  let code := [
+    Bytecode.CopyLoc 0;
+    Bytecode.MoveFromGenericDeprecated (StructDefInstantiationIndex.Build_t 0)
+  ] in
+  let module := make_module_with_local code SignatureToken.Address in
+  let module := add_simple_struct_generic_with_abilities module AbilitySet.PRIMITIVES SignatureToken.U32 in
+  let! fun_context := get_fun_context module in
+  assert_major_status
+    (verify module fun_context)
+    (fun status =>
+      match status with
+      | StatusCode.MOVEFROM_WITHOUT_KEY_ABILITY => true
+      | _ => false
+      end
+    ).
+
+Goal test_move_from_generic_deprecated_no_key = return! tt.
+Proof. reflexivity. Qed.
+
+(*
+#[test]
+#[should_panic]
+fn test_move_from_generic_deprecated_no_arg() {
+    let code = vec![Bytecode::MoveFromGenericDeprecated(
+        StructDefInstantiationIndex(0),
+    )];
+    let mut module = make_module_with_local(code, SignatureToken::Address);
+    add_simple_struct_generic_with_abilities(&mut module, AbilitySet::ALL, SignatureToken::U32);
+    let fun_context = get_fun_context(&module);
+    let _result = type_safety::verify(&module, &fun_context, &mut DummyMeter);
+}
+*)
+Definition test_move_from_generic_deprecated_no_arg : M!? _ unit :=
+  let code := [Bytecode.MoveFromGenericDeprecated (StructDefInstantiationIndex.Build_t 0)] in
+  let module := make_module_with_local code SignatureToken.Address in
+  let module := add_simple_struct_generic_with_abilities module AbilitySet.ALL SignatureToken.U32 in
+  let! fun_context := get_fun_context module in
+  verify module fun_context.
+
+Goal
+  exists (Error : Set) (error : Error),
+  test_move_from_generic_deprecated_no_arg = panic! error.
+Proof. repeat eexists. Qed.
+
+(*
+#[test]
+fn test_move_to_deprecated_correct_type() {
+    let code = vec![
+        Bytecode::ImmBorrowLoc(0),
+        Bytecode::LdU32(42),
+        Bytecode::Pack(StructDefinitionIndex(0)),
+        Bytecode::MoveToDeprecated(StructDefinitionIndex(0)),
+    ];
+    let mut module = make_module_with_local(code, SignatureToken::Signer);
+    add_simple_struct_with_abilities(&mut module, AbilitySet::ALL);
+    let fun_context = get_fun_context(&module);
+    let result = type_safety::verify(&module, &fun_context, &mut DummyMeter);
+    assert!(result.is_ok());
+}
+*)
+Definition test_move_to_deprecated_correct_type : M! unit :=
+  let code := [
+    Bytecode.ImmBorrowLoc 0;
+    Bytecode.LdU32 42;
+    Bytecode.Pack (StructDefinitionIndex.Build_t 0);
+    Bytecode.MoveToDeprecated (StructDefinitionIndex.Build_t 0)
+  ] in
+  let module := make_module_with_local code SignatureToken.Signer in
+  let module := add_simple_struct_with_abilities module AbilitySet.ALL in
+  let! fun_context := get_fun_context module in
+  let! result := verify module fun_context in
+  assert_is_ok result.
+
+Goal test_move_to_deprecated_correct_type = return! tt.
+Proof. reflexivity. Qed.
+
+(*
+#[test]
+fn test_move_to_deprecated_mismatched_types() {
+    let code = vec![
+        Bytecode::ImmBorrowLoc(0),
+        Bytecode::LdU32(42),
+        Bytecode::MoveToDeprecated(StructDefinitionIndex(0)),
+    ];
+    let mut module = make_module_with_local(code, SignatureToken::Signer);
+    add_simple_struct_with_abilities(&mut module, AbilitySet::ALL);
+    let fun_context = get_fun_context(&module);
+    let result = type_safety::verify(&module, &fun_context, &mut DummyMeter);
+    assert_eq!(
+        result.unwrap_err().major_status(),
+        StatusCode::MOVETO_TYPE_MISMATCH_ERROR
+    );
+}
+*)
+Definition test_move_to_deprecated_mismatched_types : M! unit :=
+  let code := [
+    Bytecode.ImmBorrowLoc 0;
+    Bytecode.LdU32 42;
+    Bytecode.MoveToDeprecated (StructDefinitionIndex.Build_t 0)
+  ] in
+  let module := make_module_with_local code SignatureToken.Signer in
+  let module := add_simple_struct_with_abilities module AbilitySet.ALL in
+  let! fun_context := get_fun_context module in
+  assert_major_status
+    (verify module fun_context)
+    (fun status =>
+      match status with
+      | StatusCode.MOVETO_TYPE_MISMATCH_ERROR => true
+      | _ => false
+      end
+    ).
+
+Goal test_move_to_deprecated_mismatched_types = return! tt.
+Proof. reflexivity. Qed.
+
+(*
+#[test]
+fn test_move_to_deprecated_wrong_type() {
+    let code = vec![
+        Bytecode::MutBorrowLoc(0),
+        Bytecode::LdU32(42),
+        Bytecode::Pack(StructDefinitionIndex(0)),
+        Bytecode::MoveToDeprecated(StructDefinitionIndex(0)),
+    ];
+    let mut module = make_module_with_local(code, SignatureToken::Signer);
+    add_simple_struct_with_abilities(&mut module, AbilitySet::ALL);
+    let fun_context = get_fun_context(&module);
+    let result = type_safety::verify(&module, &fun_context, &mut DummyMeter);
+    assert_eq!(
+        result.unwrap_err().major_status(),
+        StatusCode::MOVETO_TYPE_MISMATCH_ERROR
+    );
+
+    let code = vec![
+        Bytecode::ImmBorrowLoc(0),
+        Bytecode::LdU32(42),
+        Bytecode::Pack(StructDefinitionIndex(0)),
+        Bytecode::MoveToDeprecated(StructDefinitionIndex(0)),
+    ];
+    let mut module = make_module_with_local(code, SignatureToken::U32);
+    add_simple_struct_with_abilities(&mut module, AbilitySet::ALL);
+    let fun_context = get_fun_context(&module);
+    let result = type_safety::verify(&module, &fun_context, &mut DummyMeter);
+    assert_eq!(
+        result.unwrap_err().major_status(),
+        StatusCode::MOVETO_TYPE_MISMATCH_ERROR
+    );
+}
+*)
+Definition test_move_to_deprecated_wrong_type : M! unit :=
+  let code := [
+    Bytecode.MutBorrowLoc 0;
+    Bytecode.LdU32 42;
+    Bytecode.Pack (StructDefinitionIndex.Build_t 0);
+    Bytecode.MoveToDeprecated (StructDefinitionIndex.Build_t 0)
+  ] in
+  let module := make_module_with_local code SignatureToken.Signer in
+  let module := add_simple_struct_with_abilities module AbilitySet.ALL in
+  let! fun_context := get_fun_context module in
+  do! assert_major_status
+    (verify module fun_context)
+    (fun status =>
+      match status with
+      | StatusCode.MOVETO_TYPE_MISMATCH_ERROR => true
+      | _ => false
+      end
+    ) in
+  let code := [
+    Bytecode.ImmBorrowLoc 0;
+    Bytecode.LdU32 42;
+    Bytecode.Pack (StructDefinitionIndex.Build_t 0);
+    Bytecode.MoveToDeprecated (StructDefinitionIndex.Build_t 0)
+  ] in
+  let module := make_module_with_local code SignatureToken.U32 in
+  let module := add_simple_struct_with_abilities module AbilitySet.ALL in
+  let! fun_context := get_fun_context module in
+  assert_major_status
+    (verify module fun_context)
+    (fun status =>
+      match status with
+      | StatusCode.MOVETO_TYPE_MISMATCH_ERROR => true
+      | _ => false
+      end
+    ).
+
+Goal test_move_to_deprecated_wrong_type = return! tt.
+Proof. reflexivity. Qed.
+
+(*
+#[test]
+fn test_move_to_deprecated_no_key() {
+    let code = vec![
+        Bytecode::ImmBorrowLoc(0),
+        Bytecode::LdU32(42),
+        Bytecode::Pack(StructDefinitionIndex(0)),
+        Bytecode::MoveToDeprecated(StructDefinitionIndex(0)),
+    ];
+    let mut module = make_module_with_local(code, SignatureToken::Signer);
+    add_simple_struct_with_abilities(&mut module, AbilitySet::PRIMITIVES);
+    let fun_context = get_fun_context(&module);
+    let result = type_safety::verify(&module, &fun_context, &mut DummyMeter);
+    assert_eq!(
+        result.unwrap_err().major_status(),
+        StatusCode::MOVETO_WITHOUT_KEY_ABILITY
+    );
+}
+*)
+Definition test_move_to_deprecated_no_key : M! unit :=
+  let code := [
+    Bytecode.ImmBorrowLoc 0;
+    Bytecode.LdU32 42;
+    Bytecode.Pack (StructDefinitionIndex.Build_t 0);
+    Bytecode.MoveToDeprecated (StructDefinitionIndex.Build_t 0)
+  ] in
+  let module := make_module_with_local code SignatureToken.Signer in
+  let module := add_simple_struct_with_abilities module AbilitySet.PRIMITIVES in
+  let! fun_context := get_fun_context module in
+  assert_major_status
+    (verify module fun_context)
+    (fun status =>
+      match status with
+      | StatusCode.MOVETO_WITHOUT_KEY_ABILITY => true
+      | _ => false
+      end
+    ).
+
+Goal test_move_to_deprecated_no_key = return! tt.
+Proof. reflexivity. Qed.
+
+(*
+#[test]
+#[should_panic]
+fn test_move_to_too_few_args() {
+    let code = vec![
+        Bytecode::ImmBorrowLoc(0),
+        Bytecode::MoveToDeprecated(StructDefinitionIndex(0)),
+    ];
+    let mut module = make_module_with_local(code, SignatureToken::Signer);
+    add_simple_struct_with_abilities(&mut module, AbilitySet::ALL);
+    let fun_context = get_fun_context(&module);
+    let _result = type_safety::verify(&module, &fun_context, &mut DummyMeter);
+}
+*)
+Definition test_move_to_too_few_args : M!? _ unit :=
+  let code := [
+    Bytecode.ImmBorrowLoc 0;
+    Bytecode.MoveToDeprecated (StructDefinitionIndex.Build_t 0)
+  ] in
+  let module := make_module_with_local code SignatureToken.Signer in
+  let module := add_simple_struct_with_abilities module AbilitySet.ALL in
+  let! fun_context := get_fun_context module in
+  verify module fun_context.
+
+Goal
+  exists (Error : Set) (error : Error),
+  test_move_to_too_few_args = panic! error.
+Proof. repeat eexists. Qed.
+
+(*
+#[test]
+#[should_panic]
+fn test_move_to_deprecated_no_arg() {
+    let code = vec![Bytecode::MoveToDeprecated(StructDefinitionIndex(0))];
+    let mut module = make_module_with_local(code, SignatureToken::Signer);
+    add_simple_struct_with_abilities(&mut module, AbilitySet::ALL);
+    let fun_context = get_fun_context(&module);
+    let _result = type_safety::verify(&module, &fun_context, &mut DummyMeter);
+}
+*)
+Definition test_move_to_deprecated_no_arg : M!? _ unit :=
+  let code := [Bytecode.MoveToDeprecated (StructDefinitionIndex.Build_t 0)] in
+  let module := make_module_with_local code SignatureToken.Signer in
+  let module := add_simple_struct_with_abilities module AbilitySet.ALL in
+  let! fun_context := get_fun_context module in
+  verify module fun_context.
+
+Goal
+  exists (Error : Set) (error : Error),
+  test_move_to_deprecated_no_arg = panic! error.
+Proof. repeat eexists. Qed.
+
+(*
+#[test]
+fn test_move_to_generic_deprecated_correct_type() {
+    let code = vec![
+        Bytecode::ImmBorrowLoc(0),
+        Bytecode::LdU32(42),
+        Bytecode::PackGeneric(StructDefInstantiationIndex(0)),
+        Bytecode::MoveToGenericDeprecated(StructDefInstantiationIndex(0)),
+    ];
+    let mut module = make_module_with_local(code, SignatureToken::Signer);
+    add_simple_struct_generic_with_abilities(&mut module, AbilitySet::ALL, SignatureToken::U32);
+    let fun_context = get_fun_context(&module);
+    let result = type_safety::verify(&module, &fun_context, &mut DummyMeter);
+    assert!(result.is_ok());
+}
+*)
+Definition test_move_to_generic_deprecated_correct_type : M! unit :=
+  let code := [
+    Bytecode.ImmBorrowLoc 0;
+    Bytecode.LdU32 42;
+    Bytecode.PackGeneric (StructDefInstantiationIndex.Build_t 0);
+    Bytecode.MoveToGenericDeprecated (StructDefInstantiationIndex.Build_t 0)
+  ] in
+  let module := make_module_with_local code SignatureToken.Signer in
+  let module := add_simple_struct_generic_with_abilities module AbilitySet.ALL SignatureToken.U32 in
+  let! fun_context := get_fun_context module in
+  let! result := verify module fun_context in
+  assert_is_ok result.
+
+Goal test_move_to_generic_deprecated_correct_type = return! tt.
+Proof. reflexivity. Qed.
+
+(*
+#[test]
+fn test_move_to_generic_deprecated_mismatched_types() {
+    let code = vec![
+        Bytecode::ImmBorrowLoc(0),
+        Bytecode::LdU32(42),
+        Bytecode::MoveToGenericDeprecated(StructDefInstantiationIndex(0)),
+    ];
+    let mut module = make_module_with_local(code, SignatureToken::Signer);
+    add_simple_struct_generic_with_abilities(&mut module, AbilitySet::ALL, SignatureToken::U32);
+    let fun_context = get_fun_context(&module);
+    let result = type_safety::verify(&module, &fun_context, &mut DummyMeter);
+    assert_eq!(
+        result.unwrap_err().major_status(),
+        StatusCode::MOVETO_TYPE_MISMATCH_ERROR
+    );
+}
+*)
+Definition test_move_to_generic_deprecated_mismatched_types : M! unit :=
+  let code := [
+    Bytecode.ImmBorrowLoc 0;
+    Bytecode.LdU32 42;
+    Bytecode.MoveToGenericDeprecated (StructDefInstantiationIndex.Build_t 0)
+  ] in
+  let module := make_module_with_local code SignatureToken.Signer in
+  let module := add_simple_struct_generic_with_abilities module AbilitySet.ALL SignatureToken.U32 in
+  let! fun_context := get_fun_context module in
+  assert_major_status
+    (verify module fun_context)
+    (fun status =>
+      match status with
+      | StatusCode.MOVETO_TYPE_MISMATCH_ERROR => true
+      | _ => false
+      end
+    ).
+
+Goal test_move_to_generic_deprecated_mismatched_types = return! tt.
+Proof. reflexivity. Qed.
+
+(*
+#[test]
+fn test_move_to_generic_deprecated_wrong_type() {
+    let code = vec![
+        Bytecode::MutBorrowLoc(0),
+        Bytecode::LdU32(42),
+        Bytecode::PackGeneric(StructDefInstantiationIndex(0)),
+        Bytecode::MoveToGenericDeprecated(StructDefInstantiationIndex(0)),
+    ];
+    let mut module = make_module_with_local(code, SignatureToken::Signer);
+    add_simple_struct_generic_with_abilities(&mut module, AbilitySet::ALL, SignatureToken::U32);
+    let fun_context = get_fun_context(&module);
+    let result = type_safety::verify(&module, &fun_context, &mut DummyMeter);
+    assert_eq!(
+        result.unwrap_err().major_status(),
+        StatusCode::MOVETO_TYPE_MISMATCH_ERROR
+    );
+
+    let code = vec![
+        Bytecode::ImmBorrowLoc(0),
+        Bytecode::LdU32(42),
+        Bytecode::PackGeneric(StructDefInstantiationIndex(0)),
+        Bytecode::MoveToGenericDeprecated(StructDefInstantiationIndex(0)),
+    ];
+    let mut module = make_module_with_local(code, SignatureToken::U32);
+    add_simple_struct_generic_with_abilities(&mut module, AbilitySet::ALL, SignatureToken::U32);
+    let fun_context = get_fun_context(&module);
+    let result = type_safety::verify(&module, &fun_context, &mut DummyMeter);
+    assert_eq!(
+        result.unwrap_err().major_status(),
+        StatusCode::MOVETO_TYPE_MISMATCH_ERROR
+    );
+}
+*)
+Definition test_move_to_generic_deprecated_wrong_type : M! unit :=
+  let code := [
+    Bytecode.MutBorrowLoc 0;
+    Bytecode.LdU32 42;
+    Bytecode.PackGeneric (StructDefInstantiationIndex.Build_t 0);
+    Bytecode.MoveToGenericDeprecated (StructDefInstantiationIndex.Build_t 0)
+  ] in
+  let module := make_module_with_local code SignatureToken.Signer in
+  let module := add_simple_struct_generic_with_abilities module AbilitySet.ALL SignatureToken.U32 in
+  let! fun_context := get_fun_context module in
+  do! assert_major_status
+    (verify module fun_context)
+    (fun status =>
+      match status with
+      | StatusCode.MOVETO_TYPE_MISMATCH_ERROR => true
+      | _ => false
+      end
+    ) in
+  let code := [
+    Bytecode.ImmBorrowLoc 0;
+    Bytecode.LdU32 42;
+    Bytecode.PackGeneric (StructDefInstantiationIndex.Build_t 0);
+    Bytecode.MoveToGenericDeprecated (StructDefInstantiationIndex.Build_t 0)
+  ] in
+  let module := make_module_with_local code SignatureToken.U32 in
+  let module := add_simple_struct_generic_with_abilities module AbilitySet.ALL SignatureToken.U32 in
+  let! fun_context := get_fun_context module in
+  assert_major_status
+    (verify module fun_context)
+    (fun status =>
+      match status with
+      | StatusCode.MOVETO_TYPE_MISMATCH_ERROR => true
+      | _ => false
+      end
+    ).
+
+Goal test_move_to_generic_deprecated_wrong_type = return! tt.
+Proof. reflexivity. Qed.
+
+(*
+#[test]
+fn test_move_to_generic_deprecated_no_key() {
+    let code = vec![
+        Bytecode::ImmBorrowLoc(0),
+        Bytecode::LdU32(42),
+        Bytecode::PackGeneric(StructDefInstantiationIndex(0)),
+        Bytecode::MoveToGenericDeprecated(StructDefInstantiationIndex(0)),
+    ];
+    let mut module = make_module_with_local(code, SignatureToken::Signer);
+    add_simple_struct_generic_with_abilities(
+        &mut module,
+        AbilitySet::PRIMITIVES,
+        SignatureToken::U32,
+    );
+    let fun_context = get_fun_context(&module);
+    let result = type_safety::verify(&module, &fun_context, &mut DummyMeter);
+    assert_eq!(
+        result.unwrap_err().major_status(),
+        StatusCode::MOVETO_WITHOUT_KEY_ABILITY
+    );
+}
+*)
+Definition test_move_to_generic_deprecated_no_key : M! unit :=
+  let code := [
+    Bytecode.ImmBorrowLoc 0;
+    Bytecode.LdU32 42;
+    Bytecode.PackGeneric (StructDefInstantiationIndex.Build_t 0);
+    Bytecode.MoveToGenericDeprecated (StructDefInstantiationIndex.Build_t 0)
+  ] in
+  let module := make_module_with_local code SignatureToken.Signer in
+  let module := add_simple_struct_generic_with_abilities module AbilitySet.PRIMITIVES SignatureToken.U32 in
+  let! fun_context := get_fun_context module in
+  assert_major_status
+    (verify module fun_context)
+    (fun status =>
+      match status with
+      | StatusCode.MOVETO_WITHOUT_KEY_ABILITY => true
+      | _ => false
+      end
+    ).
+
+Goal test_move_to_generic_deprecated_no_key = return! tt.
+Proof. reflexivity. Qed.
+
+(*
+#[test]
+#[should_panic]
+fn test_move_to_generic_deprecated_too_few_args() {
+    let code = vec![
+        Bytecode::ImmBorrowLoc(0),
+        Bytecode::MoveToGenericDeprecated(StructDefInstantiationIndex(0)),
+    ];
+    let mut module = make_module_with_local(code, SignatureToken::Signer);
+    add_simple_struct_generic_with_abilities(&mut module, AbilitySet::ALL, SignatureToken::U32);
+    let fun_context = get_fun_context(&module);
+    let _result = type_safety::verify(&module, &fun_context, &mut DummyMeter);
+}
+*)
+Definition test_move_to_generic_deprecated_too_few_args : M!? _ unit :=
+  let code := [
+    Bytecode.ImmBorrowLoc 0;
+    Bytecode.MoveToGenericDeprecated (StructDefInstantiationIndex.Build_t 0)
+  ] in
+  let module := make_module_with_local code SignatureToken.Signer in
+  let module := add_simple_struct_generic_with_abilities module AbilitySet.ALL SignatureToken.U32 in
+  let! fun_context := get_fun_context module in
+  verify module fun_context.
+
+Goal
+  exists (Error : Set) (error : Error),
+  test_move_to_generic_deprecated_too_few_args = panic! error.
+Proof. repeat eexists. Qed.
+
+(*
+#[test]
+#[should_panic]
+fn test_move_to_generic_deprecated_no_arg() {
+    let code = vec![Bytecode::MoveToGenericDeprecated(
+        StructDefInstantiationIndex(0),
+    )];
+    let mut module = make_module_with_local(code, SignatureToken::Signer);
+    add_simple_struct_generic_with_abilities(&mut module, AbilitySet::ALL, SignatureToken::U32);
+    let fun_context = get_fun_context(&module);
+    let _result = type_safety::verify(&module, &fun_context, &mut DummyMeter);
+}
+*)
+Definition test_move_to_generic_deprecated_no_arg : M!? _ unit :=
+  let code := [Bytecode.MoveToGenericDeprecated (StructDefInstantiationIndex.Build_t 0)] in
+  let module := make_module_with_local code SignatureToken.Signer in
+  let module := add_simple_struct_generic_with_abilities module AbilitySet.ALL SignatureToken.U32 in
+  let! fun_context := get_fun_context module in
+  verify module fun_context.
+
+Goal
+  exists (Error : Set) (error : Error),
+  test_move_to_generic_deprecated_no_arg = panic! error.
+Proof. repeat eexists. Qed.
+
+(*
+#[test]
+fn test_borrow_global_deprecated_correct_type() {
+    for instr in vec![
+        Bytecode::ImmBorrowGlobalDeprecated(StructDefinitionIndex(0)),
+        Bytecode::MutBorrowGlobalDeprecated(StructDefinitionIndex(0)),
+    ] {
+        let code = vec![Bytecode::CopyLoc(0), instr];
+        let mut module = make_module_with_local(code, SignatureToken::Address);
+        add_simple_struct_with_abilities(&mut module, AbilitySet::ALL);
+        let fun_context = get_fun_context(&module);
+        let result = type_safety::verify(&module, &fun_context, &mut DummyMeter);
+        assert!(result.is_ok());
+    }
+}
+*)
+Definition test_borrow_global_deprecated_correct_type (instr : Bytecode.t) : M! unit :=
+  let code := [
+    Bytecode.CopyLoc 0;
+    instr
+  ] in
+  let module := make_module_with_local code SignatureToken.Address in
+  let module := add_simple_struct_with_abilities module AbilitySet.ALL in
+  let! fun_context := get_fun_context module in
+  let! result := verify module fun_context in
+  assert_is_ok result.
+
+Goal List.Forall
+  (fun instr => test_borrow_global_deprecated_correct_type instr = return! tt)
+  [
+    Bytecode.ImmBorrowGlobalDeprecated (StructDefinitionIndex.Build_t 0);
+    Bytecode.MutBorrowGlobalDeprecated (StructDefinitionIndex.Build_t 0)
+  ].
+Proof. repeat constructor. Qed.
+
+
+(*
+#[test]
+fn test_borrow_global_deprecated_wrong_type() {
+    for instr in vec![
+        Bytecode::ImmBorrowGlobalDeprecated(StructDefinitionIndex(0)),
+        Bytecode::MutBorrowGlobalDeprecated(StructDefinitionIndex(0)),
+    ] {
+        let code = vec![Bytecode::LdU64(42), instr];
+        let mut module = make_module_with_local(code, SignatureToken::Address);
+        add_simple_struct_with_abilities(&mut module, AbilitySet::ALL);
+        let fun_context = get_fun_context(&module);
+        let result = type_safety::verify(&module, &fun_context, &mut DummyMeter);
+        assert_eq!(
+            result.unwrap_err().major_status(),
+            StatusCode::BORROWGLOBAL_TYPE_MISMATCH_ERROR
+        );
+    }
+}
+*)
+Definition test_borrow_global_deprecated_wrong_type (instr : Bytecode.t) : M! unit :=
+  let code := [
+    Bytecode.LdU64 42;
+    instr
+  ] in
+  let module := make_module_with_local code SignatureToken.Address in
+  let module := add_simple_struct_with_abilities module AbilitySet.ALL in
+  let! fun_context := get_fun_context module in
+  assert_major_status
+    (verify module fun_context)
+    (fun status =>
+      match status with
+      | StatusCode.BORROWGLOBAL_TYPE_MISMATCH_ERROR => true
+      | _ => false
+      end
+    ).
+
+Goal List.Forall
+  (fun instr => test_borrow_global_deprecated_wrong_type instr = return! tt)
+  [
+    Bytecode.ImmBorrowGlobalDeprecated (StructDefinitionIndex.Build_t 0);
+    Bytecode.MutBorrowGlobalDeprecated (StructDefinitionIndex.Build_t 0)
+  ].
+Proof. repeat constructor. Qed.
+
+(*
+#[test]
+fn test_borrow_global_deprecated_no_key() {
+    for instr in vec![
+        Bytecode::ImmBorrowGlobalDeprecated(StructDefinitionIndex(0)),
+        Bytecode::MutBorrowGlobalDeprecated(StructDefinitionIndex(0)),
+    ] {
+        let code = vec![Bytecode::CopyLoc(0), instr];
+        let mut module = make_module_with_local(code, SignatureToken::Address);
+        add_simple_struct_with_abilities(&mut module, AbilitySet::PRIMITIVES);
+        let fun_context = get_fun_context(&module);
+        let result = type_safety::verify(&module, &fun_context, &mut DummyMeter);
+        assert_eq!(
+            result.unwrap_err().major_status(),
+            StatusCode::BORROWGLOBAL_WITHOUT_KEY_ABILITY
+        );
+    }
+}
+*)
+Definition test_borrow_global_deprecated_no_key (instr : Bytecode.t) : M! unit :=
+  let code := [
+    Bytecode.CopyLoc 0;
+    instr
+  ] in
+  let module := make_module_with_local code SignatureToken.Address in
+  let module := add_simple_struct_with_abilities module AbilitySet.PRIMITIVES in
+  let! fun_context := get_fun_context module in
+  assert_major_status
+    (verify module fun_context)
+    (fun status =>
+      match status with
+      | StatusCode.BORROWGLOBAL_WITHOUT_KEY_ABILITY => true
+      | _ => false
+      end
+    ).
+
+Goal List.Forall
+  (fun instr => test_borrow_global_deprecated_no_key instr = return! tt)
+  [
+    Bytecode.ImmBorrowGlobalDeprecated (StructDefinitionIndex.Build_t 0);
+    Bytecode.MutBorrowGlobalDeprecated (StructDefinitionIndex.Build_t 0)
+  ].
+Proof. repeat constructor. Qed.
+
+(*
+#[test]
+#[should_panic]
+fn test_borrow_global_deprecated_no_arg() {
+    for instr in vec![
+        Bytecode::ImmBorrowGlobalDeprecated(StructDefinitionIndex(0)),
+        Bytecode::MutBorrowGlobalDeprecated(StructDefinitionIndex(0)),
+    ] {
+        let code = vec![instr];
+        let mut module = make_module_with_local(code, SignatureToken::Address);
+        add_simple_struct_with_abilities(&mut module, AbilitySet::ALL);
+        let fun_context = get_fun_context(&module);
+        let _result = type_safety::verify(&module, &fun_context, &mut DummyMeter);
+    }
+}
+*)
+Definition test_borrow_global_deprecated_no_arg : M!? _ unit :=
+  let code := [Bytecode.ImmBorrowGlobalDeprecated (StructDefinitionIndex.Build_t 0)] in
+  let module := make_module_with_local code SignatureToken.Address in
+  let module := add_simple_struct_with_abilities module AbilitySet.ALL in
+  let! fun_context := get_fun_context module in
+  verify module fun_context.
+
+Goal
+  exists (Error : Set) (error : Error),
+  test_borrow_global_deprecated_no_arg = panic! error.
+Proof. repeat eexists. Qed.
+
+(*
+#[test]
+fn test_borrow_global_generic_deprecated_correct_type() {
+    for instr in vec![
+        Bytecode::ImmBorrowGlobalGenericDeprecated(StructDefInstantiationIndex(0)),
+        Bytecode::MutBorrowGlobalGenericDeprecated(StructDefInstantiationIndex(0)),
+    ] {
+        let code = vec![Bytecode::CopyLoc(0), instr];
+        let mut module = make_module_with_local(code, SignatureToken::Address);
+        add_simple_struct_generic_with_abilities(&mut module, AbilitySet::ALL, SignatureToken::U32);
+        let fun_context = get_fun_context(&module);
+        let result = type_safety::verify(&module, &fun_context, &mut DummyMeter);
+        assert!(result.is_ok());
+    }
+}
+*)
+Definition test_borrow_global_generic_deprecated_correct_type (instr : Bytecode.t) : M! unit :=
+  let code := [
+    Bytecode.CopyLoc 0;
+    instr
+  ] in
+  let module := make_module_with_local code SignatureToken.Address in
+  let module := add_simple_struct_generic_with_abilities module AbilitySet.ALL SignatureToken.U32 in
+  let! fun_context := get_fun_context module in
+  let! result := verify module fun_context in
+  assert_is_ok result.
+
+Goal List.Forall
+  (fun instr => test_borrow_global_generic_deprecated_correct_type instr = return! tt)
+  [
+    Bytecode.ImmBorrowGlobalGenericDeprecated (StructDefInstantiationIndex.Build_t 0);
+    Bytecode.MutBorrowGlobalGenericDeprecated (StructDefInstantiationIndex.Build_t 0)
+  ].
+Proof. repeat constructor. Qed.
+
+(*
+#[test]
+fn test_borrow_global_generic_deprecated_wrong_type() {
+    for instr in vec![
+        Bytecode::ImmBorrowGlobalGenericDeprecated(StructDefInstantiationIndex(0)),
+        Bytecode::MutBorrowGlobalGenericDeprecated(StructDefInstantiationIndex(0)),
+    ] {
+        let code = vec![Bytecode::LdU64(42), instr];
+        let mut module = make_module_with_local(code, SignatureToken::Address);
+        add_simple_struct_generic_with_abilities(&mut module, AbilitySet::ALL, SignatureToken::U32);
+        let fun_context = get_fun_context(&module);
+        let result = type_safety::verify(&module, &fun_context, &mut DummyMeter);
+        assert_eq!(
+            result.unwrap_err().major_status(),
+            StatusCode::BORROWGLOBAL_TYPE_MISMATCH_ERROR
+        );
+    }
+}
+*)
+Definition test_borrow_global_generic_deprecated_wrong_type (instr : Bytecode.t) : M! unit :=
+  let code := [
+    Bytecode.LdU64 42;
+    instr
+  ] in
+  let module := make_module_with_local code SignatureToken.Address in
+  let module := add_simple_struct_generic_with_abilities module AbilitySet.ALL SignatureToken.U32 in
+  let! fun_context := get_fun_context module in
+  assert_major_status
+    (verify module fun_context)
+    (fun status =>
+      match status with
+      | StatusCode.BORROWGLOBAL_TYPE_MISMATCH_ERROR => true
+      | _ => false
+      end
+    ).
+
+Goal List.Forall
+  (fun instr => test_borrow_global_generic_deprecated_wrong_type instr = return! tt)
+  [
+    Bytecode.ImmBorrowGlobalGenericDeprecated (StructDefInstantiationIndex.Build_t 0);
+    Bytecode.MutBorrowGlobalGenericDeprecated (StructDefInstantiationIndex.Build_t 0)
+  ].
+Proof. repeat constructor. Qed.
+
+(*
+#[test]
+fn test_borrow_global_generic_deprecated_no_key() {
+    for instr in vec![
+        Bytecode::ImmBorrowGlobalGenericDeprecated(StructDefInstantiationIndex(0)),
+        Bytecode::MutBorrowGlobalGenericDeprecated(StructDefInstantiationIndex(0)),
+    ] {
+        let code = vec![Bytecode::CopyLoc(0), instr];
+        let mut module = make_module_with_local(code, SignatureToken::Address);
+        add_simple_struct_generic_with_abilities(
+            &mut module,
+            AbilitySet::PRIMITIVES,
+            SignatureToken::U32,
+        );
+        let fun_context = get_fun_context(&module);
+        let result = type_safety::verify(&module, &fun_context, &mut DummyMeter);
+        assert_eq!(
+            result.unwrap_err().major_status(),
+            StatusCode::BORROWGLOBAL_WITHOUT_KEY_ABILITY
+        );
+    }
+}
+*)
+Definition test_borrow_global_generic_deprecated_no_key (instr : Bytecode.t) : M! unit :=
+  let code := [
+    Bytecode.CopyLoc 0;
+    instr
+  ] in
+  let module := make_module_with_local code SignatureToken.Address in
+  let module := add_simple_struct_generic_with_abilities module AbilitySet.PRIMITIVES SignatureToken.U32 in
+  let! fun_context := get_fun_context module in
+  assert_major_status
+    (verify module fun_context)
+    (fun status =>
+      match status with
+      | StatusCode.BORROWGLOBAL_WITHOUT_KEY_ABILITY => true
+      | _ => false
+      end
+    ).
+
+Goal List.Forall
+  (fun instr => test_borrow_global_generic_deprecated_no_key instr = return! tt)
+  [
+    Bytecode.ImmBorrowGlobalGenericDeprecated (StructDefInstantiationIndex.Build_t 0);
+    Bytecode.MutBorrowGlobalGenericDeprecated (StructDefInstantiationIndex.Build_t 0)
+  ].
+Proof. repeat constructor. Qed.
+
+(*
+#[test]
+#[should_panic]
+fn test_borrow_global_generic_deprecated_no_arg() {
+    for instr in vec![
+        Bytecode::ImmBorrowGlobalGenericDeprecated(StructDefInstantiationIndex(0)),
+        Bytecode::MutBorrowGlobalGenericDeprecated(StructDefInstantiationIndex(0)),
+    ] {
+        let code = vec![instr];
+        let mut module = make_module_with_local(code, SignatureToken::Address);
+        add_simple_struct_generic_with_abilities(&mut module, AbilitySet::ALL, SignatureToken::U32);
+        let fun_context = get_fun_context(&module);
+        let _result = type_safety::verify(&module, &fun_context, &mut DummyMeter);
+    }
+}
+*)
+Definition test_borrow_global_generic_deprecated_no_arg (instr : Bytecode.t) : M!? _ unit :=
+  let code := [instr] in
+  let module := make_module_with_local code SignatureToken.Address in
+  let module := add_simple_struct_generic_with_abilities module AbilitySet.ALL SignatureToken.U32 in
+  let! fun_context := get_fun_context module in
+  verify module fun_context.
+
+Goal
+  List.Forall
+    (fun instr =>
+      exists (Error : Set) (error : Error),
+      test_borrow_global_generic_deprecated_no_arg instr = panic! error
+    )
+    [
+      Bytecode.ImmBorrowGlobalGenericDeprecated (StructDefInstantiationIndex.Build_t 0);
+      Bytecode.MutBorrowGlobalGenericDeprecated (StructDefInstantiationIndex.Build_t 0)
+    ].
+Proof. repeat econstructor. Qed.
